Reorganizing + extraction to F# + compatibility with current F* version

src/fs/AncillaHeap.fs
@@ -1,0 +1,124 @@
+#light "off"
+module AncillaHeap
+open Prims
+
+type l__AncHeapRecord =
+{hp : PairHeap.intHeap; max : Prims.int}
+
+
+let is_MkAncHeapRecord : l__AncHeapRecord  ->  Prims.bool = (Prims.checked_cast(fun ( _  :  l__AncHeapRecord ) -> (FStar.All.failwith "Not yet implemented:is_MkAncHeapRecord")))
+
+
+type l__AncHeap =
+l__AncHeapRecord
+
+
+let emptyHeap : l__AncHeap = {hp = PairHeap.Empty; max = 0}
+
+
+let above : Prims.int  ->  l__AncHeap = (fun ( n  :  Prims.int ) -> {hp = PairHeap.Empty; max = n})
+
+
+let maxUsed : l__AncHeap  ->  Prims.int = (fun ( ah  :  l__AncHeap ) -> ah.max)
+
+
+let dat : l__AncHeap  ->  PairHeap.intHeap = (fun ( ah  :  l__AncHeap ) -> ah.hp)
+
+
+let insert : l__AncHeap  ->  Prims.int  ->  l__AncHeap = (fun ( ah  :  l__AncHeap ) ( i  :  Prims.int ) -> (
+
+let newMax = if (i < ah.max) then begin
+ah.max
+end else begin
+(i + 1)
+end
+in {hp = (PairHeap.insert ah.hp i); max = newMax}))
+
+
+let popMin : l__AncHeap  ->  (l__AncHeap * Prims.int) = (fun ( ah  :  l__AncHeap ) -> (match (ah.hp) with
+| PairHeap.Empty -> begin
+((
+
+let _14_16 = ah
+in {hp = _14_16.hp; max = (ah.max + 1)}), ah.max)
+end
+| PairHeap.Heap (r, l) -> begin
+(
+
+let hp' = (
+
+let _14_22 = ()
+in (
+
+let _14_24 = ()
+in (PairHeap.deleteMin ah.hp)))
+in ((
+
+let _14_27 = ah
+in {hp = hp'; max = _14_27.max}), (PairHeap.getMin ah.hp)))
+end))
+
+
+let rec getn_acc : l__AncHeap  ->  Prims.int Prims.list  ->  Prims.nat  ->  (l__AncHeap * Prims.int Prims.list) = (fun ( ah  :  l__AncHeap ) ( acc  :  Prims.int Prims.list ) ( n  :  Prims.nat ) -> (match (n) with
+| 0 -> begin
+(ah, acc)
+end
+| n -> begin
+(
+
+let _14_36 = (popMin ah)
+in (match (_14_36) with
+| (newah, v) -> begin
+(getn_acc newah ((v)::acc) (n - 1))
+end))
+end))
+
+
+let getn : l__AncHeap  ->  Prims.nat  ->  (l__AncHeap * Prims.int Prims.list) = (fun ( ah  :  l__AncHeap ) ( n  :  Prims.nat ) -> (getn_acc ah [] n))
+
+
+let mem : Prims.int  ->  l__AncHeap  ->  Prims.bool = (fun ( i  :  Prims.int ) ( ah  :  l__AncHeap ) -> if (i >= ah.max) then begin
+true
+end else begin
+(PairHeap.mem i ah.hp)
+end)
+
+
+let elts : l__AncHeap  ->  Prims.int Util.set = (fun ( ah  :  l__AncHeap ) ( i  :  Prims.int ) -> (mem i ah))
+
+
+let get_min : l__AncHeap  ->  Prims.int = (fun ( ah  :  l__AncHeap ) -> (Prims.snd (popMin ah)))
+
+
+let delete_min : l__AncHeap  ->  l__AncHeap = (fun ( ah  :  l__AncHeap ) -> (Prims.fst (popMin ah)))
+
+
+let pop_is_zero : Total.state  ->  l__AncHeap  ->  Prims.unit = (fun ( st  :  Total.state ) ( ah  :  l__AncHeap ) -> ())
+
+
+let max_increasing : l__AncHeap  ->  Prims.unit = (fun ( ah  :  l__AncHeap ) -> ())
+
+
+let pop_not_elt : l__AncHeap  ->  Prims.unit = (fun ( ah  :  l__AncHeap ) -> ())
+
+
+let pop_elt : l__AncHeap  ->  Prims.unit = (fun ( ah  :  l__AncHeap ) -> ())
+
+
+let pop_subset : l__AncHeap  ->  Prims.unit = (fun ( ah  :  l__AncHeap ) -> ())
+
+
+let pop_proper_subset : l__AncHeap  ->  Prims.unit = (fun ( ah  :  l__AncHeap ) -> ())
+
+
+let zeroHeap_subset : Total.state  ->  l__AncHeap  ->  l__AncHeap  ->  Prims.unit = (fun ( st  :  Total.state ) ( ah  :  l__AncHeap ) ( ah'  :  l__AncHeap ) -> ())
+
+
+let zeroHeap_insert : Total.state  ->  l__AncHeap  ->  Prims.int  ->  Prims.unit = (fun ( st  :  Total.state ) ( ah  :  l__AncHeap ) ( i  :  Prims.int ) -> ())
+
+
+let rec zeroHeap_insert_list : Total.state  ->  l__AncHeap  ->  Prims.int Prims.list  ->  Prims.unit = (fun ( st  :  Total.state ) ( ah  :  l__AncHeap ) ( lst  :  Prims.int Prims.list ) -> ())
+
+
+
+
