src/fs/BoolExp.fs
@@ -1,0 +1,754 @@
+#light "off"
+module BoolExp
+open Prims
+
+type l__BoolExp =
+| BFalse
+| BVar of Prims.int
+| BNot of l__BoolExp
+| BAnd of (l__BoolExp * l__BoolExp)
+| BXor of (l__BoolExp * l__BoolExp)
+
+
+let is_BFalse = (fun ( _discr_  :  obj ) -> (match (_discr_) with
+| BFalse (_) -> begin
+true
+end
+| _ -> begin
+false
+end))
+
+
+let is_BVar = (fun ( _discr_  :  obj ) -> (match (_discr_) with
+| BVar (_) -> begin
+true
+end
+| _ -> begin
+false
+end))
+
+
+let is_BNot = (fun ( _discr_  :  obj ) -> (match (_discr_) with
+| BNot (_) -> begin
+true
+end
+| _ -> begin
+false
+end))
+
+
+let is_BAnd = (fun ( _discr_  :  obj ) -> (match (_discr_) with
+| BAnd (_) -> begin
+true
+end
+| _ -> begin
+false
+end))
+
+
+let is_BXor = (fun ( _discr_  :  obj ) -> (match (_discr_) with
+| BXor (_) -> begin
+true
+end
+| _ -> begin
+false
+end))
+
+
+let ___BVar____0 = (fun ( projectee  :  l__BoolExp ) -> (match (projectee) with
+| BVar (_16_3) -> begin
+_16_3
+end))
+
+
+let ___BNot____0 = (fun ( projectee  :  l__BoolExp ) -> (match (projectee) with
+| BNot (_16_6) -> begin
+_16_6
+end))
+
+
+let ___BAnd____0 = (fun ( projectee  :  l__BoolExp ) -> (match (projectee) with
+| BAnd (_16_9) -> begin
+_16_9
+end))
+
+
+let ___BXor____0 = (fun ( projectee  :  l__BoolExp ) -> (match (projectee) with
+| BXor (_16_12) -> begin
+_16_12
+end))
+
+
+let rec prettyPrintBexp : l__BoolExp  ->  Prims.string = (fun ( bexp  :  l__BoolExp ) -> (match (bexp) with
+| BFalse -> begin
+"false"
+end
+| BVar (i) -> begin
+(Prims.string_of_int i)
+end
+| BNot (x) -> begin
+(FStar.String.strcat "~" (prettyPrintBexp x))
+end
+| BAnd (x, y) -> begin
+(FStar.String.strcat "(" (FStar.String.strcat (prettyPrintBexp x) (FStar.String.strcat " && " (FStar.String.strcat (prettyPrintBexp y) ")"))))
+end
+| BXor (x, y) -> begin
+(FStar.String.strcat "(" (FStar.String.strcat (prettyPrintBexp x) (FStar.String.strcat " <> " (FStar.String.strcat (prettyPrintBexp y) ")"))))
+end))
+
+
+let rec occursInBexp : Prims.int  ->  l__BoolExp  ->  Prims.bool = (fun ( i  :  Prims.int ) ( exp  :  l__BoolExp ) -> (match (exp) with
+| BFalse -> begin
+false
+end
+| BVar (n) -> begin
+(n = i)
+end
+| BAnd (x, y) -> begin
+((occursInBexp i x) || (occursInBexp i y))
+end
+| BXor (x, y) -> begin
+((occursInBexp i x) || (occursInBexp i y))
+end
+| BNot (x) -> begin
+(occursInBexp i x)
+end))
+
+
+let vars : l__BoolExp  ->  Prims.int Util.set = (fun ( exp  :  l__BoolExp ) ( i  :  Prims.int ) -> (occursInBexp i exp))
+
+
+let rec getVars_acc : Prims.int Prims.list  ->  l__BoolExp  ->  Prims.int Prims.list = (fun ( acc  :  Prims.int Prims.list ) ( exp  :  l__BoolExp ) -> (match (exp) with
+| BFalse -> begin
+[]
+end
+| BVar (n) -> begin
+if (FStar.List.memT n acc) then begin
+acc
+end else begin
+(n)::acc
+end
+end
+| BAnd (x, y) -> begin
+(getVars_acc (getVars_acc acc x) y)
+end
+| BXor (x, y) -> begin
+(getVars_acc (getVars_acc acc x) y)
+end
+| BNot (exp) -> begin
+(getVars_acc acc exp)
+end))
+
+
+let getVars : l__BoolExp  ->  Prims.int Prims.list = (fun ( exp  :  l__BoolExp ) -> (getVars_acc [] exp))
+
+
+let max : Prims.int  ->  Prims.int  ->  Prims.int = (fun ( x  :  Prims.int ) ( y  :  Prims.int ) -> if (x > y) then begin
+x
+end else begin
+y
+end)
+
+
+let rec listMax : Prims.int Prims.list  ->  Prims.int = (fun ( lst  :  Prims.int Prims.list ) -> (match (lst) with
+| [] -> begin
+0
+end
+| x::xs -> begin
+(max x (listMax xs))
+end))
+
+
+let varCount : l__BoolExp  ->  Prims.int = (fun ( exp  :  l__BoolExp ) -> (FStar.List.lengthT (getVars exp)))
+
+
+let varMax : l__BoolExp  ->  Prims.int = (fun ( exp  :  l__BoolExp ) -> (listMax (getVars exp)))
+
+
+let rec gtVars : Prims.int  ->  l__BoolExp  ->  Prims.bool = (fun ( i  :  Prims.int ) ( bexp  :  l__BoolExp ) -> (match (bexp) with
+| BFalse -> begin
+false
+end
+| BVar (j) -> begin
+(i > j)
+end
+| BNot (x) -> begin
+(gtVars i x)
+end
+| (BXor (x, y)) | (BAnd (x, y)) -> begin
+((gtVars i x) && (gtVars i y))
+end))
+
+
+let rec substBexp : l__BoolExp  ->  (Prims.int, l__BoolExp) Total.map  ->  l__BoolExp = (fun ( bexp  :  l__BoolExp ) ( sub  :  (Prims.int, l__BoolExp) Total.map ) -> (match (bexp) with
+| BFalse -> begin
+BFalse
+end
+| BVar (i) -> begin
+(sub i)
+end
+| BNot (x) -> begin
+BNot ((substBexp x sub))
+end
+| BAnd (x, y) -> begin
+BAnd (((substBexp x sub), (substBexp y sub)))
+end
+| BXor (x, y) -> begin
+BXor (((substBexp x sub), (substBexp y sub)))
+end))
+
+
+let rec substVar : l__BoolExp  ->  (Prims.int, Prims.int) Total.map  ->  l__BoolExp = (fun ( bexp  :  l__BoolExp ) ( sub  :  (Prims.int, Prims.int) Total.map ) -> (match (bexp) with
+| BFalse -> begin
+BFalse
+end
+| BVar (i) -> begin
+BVar ((sub i))
+end
+| BNot (x) -> begin
+BNot ((substVar x sub))
+end
+| BAnd (x, y) -> begin
+BAnd (((substVar x sub), (substVar y sub)))
+end
+| BXor (x, y) -> begin
+BXor (((substVar x sub), (substVar y sub)))
+end))
+
+
+let rec evalBexp : l__BoolExp  ->  Total.state  ->  Prims.bool = (fun ( bexp  :  l__BoolExp ) ( st  :  Total.state ) -> (match (bexp) with
+| BFalse -> begin
+false
+end
+| BVar (i) -> begin
+(st i)
+end
+| BNot (x) -> begin
+(not ((evalBexp x st)))
+end
+| BAnd (x, y) -> begin
+((evalBexp x st) && (evalBexp y st))
+end
+| BXor (x, y) -> begin
+((evalBexp x st) <> (evalBexp y st))
+end))
+
+
+let rec simplify : l__BoolExp  ->  l__BoolExp = (fun ( exp  :  l__BoolExp ) -> (match (exp) with
+| BFalse -> begin
+BFalse
+end
+| BVar (x) -> begin
+exp
+end
+| BAnd (x, y) -> begin
+(
+
+let x' = (simplify x)
+in (
+
+let y' = (simplify y)
+in (match ((x', y')) with
+| ((BFalse, _)) | ((_, BFalse)) -> begin
+BFalse
+end
+| _16_150 -> begin
+BAnd ((x', y'))
+end)))
+end
+| BXor (x, y) -> begin
+(
+
+let x' = (simplify x)
+in (
+
+let y' = (simplify y)
+in (match ((x', y')) with
+| ((BFalse, z)) | ((z, BFalse)) -> begin
+z
+end
+| _16_163 -> begin
+BXor ((x', y'))
+end)))
+end
+| BNot (x) -> begin
+(
+
+let x' = (simplify x)
+in (match (x') with
+| BNot (y) -> begin
+y
+end
+| _16_170 -> begin
+BNot (x')
+end))
+end))
+
+
+let rec factorAs : l__BoolExp  ->  Prims.int  ->  l__BoolExp Prims.option = (fun ( exp  :  l__BoolExp ) ( targ  :  Prims.int ) -> (match (exp) with
+| BFalse -> begin
+None
+end
+| BVar (i) -> begin
+if (i = targ) then begin
+Some (BFalse)
+end else begin
+None
+end
+end
+| BNot (x) -> begin
+(match ((factorAs x targ)) with
+| None -> begin
+None
+end
+| Some (x') -> begin
+Some (BNot (x'))
+end)
+end
+| BAnd (x, y) -> begin
+None
+end
+| BXor (x, y) -> begin
+if (not ((occursInBexp targ y))) then begin
+(match ((factorAs x targ)) with
+| None -> begin
+None
+end
+| Some (x') -> begin
+Some (BXor ((x', y)))
+end)
+end else begin
+if (not ((occursInBexp targ x))) then begin
+(match ((factorAs y targ)) with
+| None -> begin
+None
+end
+| Some (y') -> begin
+Some (BXor ((x, y')))
+end)
+end else begin
+None
+end
+end
+end))
+
+
+let rec distributeAnds : l__BoolExp  ->  l__BoolExp = (fun ( exp  :  l__BoolExp ) -> (match (exp) with
+| BFalse -> begin
+BFalse
+end
+| BVar (v) -> begin
+BVar (v)
+end
+| BNot (x) -> begin
+BNot ((distributeAnds x))
+end
+| BAnd (x, y) -> begin
+(match (((distributeAnds x), (distributeAnds y))) with
+| (BXor (a, b), BXor (c, d)) -> begin
+BXor ((BXor ((BAnd ((a, c)), BAnd ((b, c)))), BXor ((BAnd ((a, d)), BAnd ((b, d))))))
+end
+| (x', BXor (c, d)) -> begin
+BXor ((BAnd ((x', c)), BAnd ((x', d))))
+end
+| (BXor (a, b), y') -> begin
+BXor ((BAnd ((a, y')), BAnd ((b, y'))))
+end
+| (x', y') -> begin
+BAnd ((x', y'))
+end)
+end
+| BXor (x, y) -> begin
+BXor (((distributeAnds x), (distributeAnds y)))
+end))
+
+
+let rec undistributeAnds : l__BoolExp  ->  l__BoolExp = (fun ( exp  :  l__BoolExp ) -> (match (exp) with
+| BFalse -> begin
+BFalse
+end
+| BVar (v) -> begin
+BVar (v)
+end
+| BNot (x) -> begin
+BNot ((undistributeAnds x))
+end
+| BAnd (x, y) -> begin
+BAnd (((undistributeAnds x), (undistributeAnds y)))
+end
+| BXor (x, y) -> begin
+(match (((undistributeAnds x), (undistributeAnds y))) with
+| (BAnd (a, b), BAnd (c, d)) -> begin
+if (a = c) then begin
+BAnd ((a, BXor ((b, d))))
+end else begin
+if (a = d) then begin
+BAnd ((a, BXor ((b, c))))
+end else begin
+if (b = c) then begin
+BAnd ((b, BXor ((a, d))))
+end else begin
+if (b = d) then begin
+BAnd ((b, BXor ((a, c))))
+end else begin
+BXor ((BAnd ((a, b)), BAnd ((c, d))))
+end
+end
+end
+end
+end
+| (x', y') -> begin
+BXor ((x', y'))
+end)
+end))
+
+
+type compilerResult =
+(AncillaHeap.l__AncHeap * Prims.int * Prims.int Prims.list * Circuit.l__Gate Prims.list)
+
+
+let rec compileBexp : AncillaHeap.l__AncHeap  ->  Prims.int  ->  l__BoolExp  ->  compilerResult = (fun ( ah  :  AncillaHeap.l__AncHeap ) ( targ  :  Prims.int ) ( exp  :  l__BoolExp ) -> (match (exp) with
+| BFalse -> begin
+(ah, targ, [], [])
+end
+| BVar (v) -> begin
+(ah, targ, [], (Circuit.RCNOT ((v, targ)))::[])
+end
+| BAnd (x, y) -> begin
+(
+
+let _16_279 = (compileBexp_oop ah x)
+in (match (_16_279) with
+| (ah', xres, xanc, xgate) -> begin
+(
+
+let _16_284 = (compileBexp_oop ah' y)
+in (match (_16_284) with
+| (ah'', yres, yanc, ygate) -> begin
+(ah'', targ, (FStar.List.append xanc yanc), (FStar.List.append (FStar.List.append xgate ygate) ((Circuit.RTOFF ((xres, yres, targ)))::[])))
+end))
+end))
+end
+| BXor (x, y) -> begin
+(
+
+let _16_293 = (compileBexp ah targ x)
+in (match (_16_293) with
+| (ah', xres, xanc, xgate) -> begin
+(
+
+let _16_298 = (compileBexp ah' targ y)
+in (match (_16_298) with
+| (ah'', yres, yanc, ygate) -> begin
+(ah'', targ, (FStar.List.append xanc yanc), (FStar.List.append xgate ygate))
+end))
+end))
+end
+| BNot (exp) -> begin
+(
+
+let _16_305 = (compileBexp ah targ exp)
+in (match (_16_305) with
+| (ah', xres, xanc, xgate) -> begin
+(ah', targ, xanc, (FStar.List.append xgate ((Circuit.RNOT (xres))::[])))
+end))
+end))
+and compileBexp_oop : AncillaHeap.l__AncHeap  ->  l__BoolExp  ->  compilerResult = (fun ( ah  :  AncillaHeap.l__AncHeap ) ( exp  :  l__BoolExp ) -> (match (exp) with
+| BVar (v) -> begin
+(ah, v, [], [])
+end
+| _16_311 -> begin
+(
+
+let _16_314 = (AncillaHeap.popMin ah)
+in (match (_16_314) with
+| (ah', targ) -> begin
+(
+
+let _16_319 = (compileBexp ah' targ exp)
+in (match (_16_319) with
+| (ah'', res, anc, gate) -> begin
+(ah'', res, (targ)::anc, gate)
+end))
+end))
+end))
+
+
+let compileBexpClean : AncillaHeap.l__AncHeap  ->  Prims.int  ->  l__BoolExp  ->  compilerResult = (fun ( ah  :  AncillaHeap.l__AncHeap ) ( targ  :  Prims.int ) ( exp  :  l__BoolExp ) -> (
+
+let _16_327 = (compileBexp ah targ exp)
+in (match (_16_327) with
+| (ah', res, anc, circ) -> begin
+(
+
+let cleanup = (Circuit.uncompute circ res)
+in (
+
+let ah'' = (FStar.List.fold_leftT AncillaHeap.insert ah' anc)
+in (ah'', res, [], (FStar.List.append circ (FStar.List.rev cleanup)))))
+end)))
+
+
+let compileBexpClean_oop : AncillaHeap.l__AncHeap  ->  l__BoolExp  ->  compilerResult = (fun ( ah  :  AncillaHeap.l__AncHeap ) ( exp  :  l__BoolExp ) -> (match (exp) with
+| BVar (v) -> begin
+(ah, v, [], [])
+end
+| _16_335 -> begin
+(
+
+let _16_338 = (AncillaHeap.popMin ah)
+in (match (_16_338) with
+| (ah', targ) -> begin
+(
+
+let _16_343 = (compileBexpClean ah' targ exp)
+in (match (_16_343) with
+| (ah'', res, anc, gate) -> begin
+(ah'', res, (targ)::anc, gate)
+end))
+end))
+end))
+
+
+let rec compileBexpPebbled : AncillaHeap.l__AncHeap  ->  Prims.int  ->  l__BoolExp  ->  compilerResult = (fun ( ah  :  AncillaHeap.l__AncHeap ) ( targ  :  Prims.int ) ( exp  :  l__BoolExp ) -> (match (exp) with
+| BFalse -> begin
+(ah, targ, [], [])
+end
+| BVar (v) -> begin
+(ah, targ, [], (Circuit.RCNOT ((v, targ)))::[])
+end
+| BAnd (x, y) -> begin
+(
+
+let _16_360 = (compileBexpPebbled_oop ah x)
+in (match (_16_360) with
+| (ah', xres, xanc, xgate) -> begin
+(
+
+let _16_365 = (compileBexpPebbled_oop ah' y)
+in (match (_16_365) with
+| (ah'', yres, yanc, ygate) -> begin
+(
+
+let cleanup = (Circuit.uncompute (FStar.List.append xgate ygate) targ)
+in (
+
+let ah''' = (FStar.List.fold_leftT AncillaHeap.insert ah'' (FStar.List.append xanc yanc))
+in (ah''', targ, [], (FStar.List.append (FStar.List.append (FStar.List.append xgate ygate) ((Circuit.RTOFF ((xres, yres, targ)))::[])) (FStar.List.rev cleanup)))))
+end))
+end))
+end
+| BXor (x, y) -> begin
+(
+
+let _16_376 = (compileBexpPebbled ah targ x)
+in (match (_16_376) with
+| (ah', xres, xanc, xgate) -> begin
+(
+
+let _16_381 = (compileBexpPebbled ah' targ y)
+in (match (_16_381) with
+| (ah'', yres, yanc, ygate) -> begin
+(ah'', targ, (FStar.List.append xanc yanc), (FStar.List.append xgate ygate))
+end))
+end))
+end
+| BNot (exp) -> begin
+(
+
+let _16_388 = (compileBexpPebbled ah targ exp)
+in (match (_16_388) with
+| (ah', xres, xanc, xgate) -> begin
+(ah', targ, xanc, (FStar.List.append xgate ((Circuit.RNOT (xres))::[])))
+end))
+end))
+and compileBexpPebbled_oop : AncillaHeap.l__AncHeap  ->  l__BoolExp  ->  compilerResult = (fun ( ah  :  AncillaHeap.l__AncHeap ) ( exp  :  l__BoolExp ) -> (match (exp) with
+| BVar (v) -> begin
+(ah, v, [], [])
+end
+| _16_394 -> begin
+(
+
+let _16_397 = (AncillaHeap.popMin ah)
+in (match (_16_397) with
+| (ah', targ) -> begin
+(
+
+let _16_402 = (compileBexpPebbled ah' targ exp)
+in (match (_16_402) with
+| (ah'', res, anc, gate) -> begin
+(ah'', res, (targ)::anc, gate)
+end))
+end))
+end))
+
+
+let first = (fun ( _16_410  :  ('A_16_82024 * 'A_16_82023 * 'A_16_82022 * 'A_16_82021) ) -> (match (_16_410) with
+| (x, _16_405, _16_407, _16_409) -> begin
+x
+end))
+
+
+let second = (fun ( _16_418  :  ('A_16_82160 * 'A_16_82159 * 'A_16_82158 * 'A_16_82157) ) -> (match (_16_418) with
+| (_16_412, x, _16_415, _16_417) -> begin
+x
+end))
+
+
+let third = (fun ( _16_426  :  ('A_16_82296 * 'A_16_82295 * 'A_16_82294 * 'A_16_82293) ) -> (match (_16_426) with
+| (_16_420, _16_422, x, _16_425) -> begin
+x
+end))
+
+
+let last = (fun ( _16_434  :  ('A_16_82432 * 'A_16_82431 * 'A_16_82430 * 'A_16_82429) ) -> (match (_16_434) with
+| (_16_428, _16_430, _16_432, x) -> begin
+x
+end))
+
+
+let compileBexpEval : AncillaHeap.l__AncHeapRecord  ->  Prims.int  ->  l__BoolExp  ->  Total.state  ->  Prims.bool = (fun ( ah  :  AncillaHeap.l__AncHeapRecord ) ( targ  :  Prims.int ) ( exp  :  l__BoolExp ) ( st  :  Total.state ) -> (
+
+let _16_443 = (compileBexp ah targ exp)
+in (match (_16_443) with
+| (ah', res, anc, circ) -> begin
+(Circuit.evalCirc circ st res)
+end)))
+
+
+let compileBexpEval_oop : AncillaHeap.l__AncHeapRecord  ->  l__BoolExp  ->  Total.state  ->  Prims.bool = (fun ( ah  :  AncillaHeap.l__AncHeapRecord ) ( exp  :  l__BoolExp ) ( st  :  Total.state ) -> (
+
+let _16_451 = (compileBexp_oop ah exp)
+in (match (_16_451) with
+| (ah', res, anc, circ) -> begin
+(Circuit.evalCirc circ st res)
+end)))
+
+
+let compileBexpCleanEval : AncillaHeap.l__AncHeapRecord  ->  Prims.int  ->  l__BoolExp  ->  Total.state  ->  Prims.bool = (fun ( ah  :  AncillaHeap.l__AncHeapRecord ) ( targ  :  Prims.int ) ( exp  :  l__BoolExp ) ( st  :  Total.state ) -> (
+
+let _16_460 = (compileBexpClean ah targ exp)
+in (match (_16_460) with
+| (ah', res, anc, circ) -> begin
+(Circuit.evalCirc circ st res)
+end)))
+
+
+let compileBexpCleanEval_oop : AncillaHeap.l__AncHeapRecord  ->  l__BoolExp  ->  Total.state  ->  Prims.bool = (fun ( ah  :  AncillaHeap.l__AncHeapRecord ) ( exp  :  l__BoolExp ) ( st  :  Total.state ) -> (
+
+let _16_468 = (compileBexpClean_oop ah exp)
+in (match (_16_468) with
+| (ah', res, anc, circ) -> begin
+(Circuit.evalCirc circ st res)
+end)))
+
+
+let compileBexpCleanEvalSt : AncillaHeap.l__AncHeapRecord  ->  Prims.int  ->  l__BoolExp  ->  Total.state  ->  Total.state = (fun ( ah  :  AncillaHeap.l__AncHeapRecord ) ( targ  :  Prims.int ) ( exp  :  l__BoolExp ) ( st  :  Total.state ) -> (
+
+let _16_477 = (compileBexpClean ah targ exp)
+in (match (_16_477) with
+| (ah', res, anc, circ) -> begin
+(Circuit.evalCirc circ st)
+end)))
+
+
+let compileBexpCleanEvalSt_oop : AncillaHeap.l__AncHeapRecord  ->  l__BoolExp  ->  Total.state  ->  Total.state = (fun ( ah  :  AncillaHeap.l__AncHeapRecord ) ( exp  :  l__BoolExp ) ( st  :  Total.state ) -> (
+
+let _16_485 = (compileBexpClean_oop ah exp)
+in (match (_16_485) with
+| (ah', res, anc, circ) -> begin
+(Circuit.evalCirc circ st)
+end)))
+
+
+let rec simplify_preserves_semantics : l__BoolExp  ->  Prims.unit = (fun ( exp  :  l__BoolExp ) -> ())
+
+
+let rec factorAs_correct : l__BoolExp  ->  Prims.int  ->  Total.state  ->  Prims.unit = (fun ( exp  :  l__BoolExp ) ( targ  :  Prims.int ) ( st  :  Total.state ) -> ())
+
+
+let rec factorAs_vars : l__BoolExp  ->  Prims.int  ->  Prims.unit = (fun ( exp  :  l__BoolExp ) ( targ  :  Prims.int ) -> ())
+
+
+let idempotentAnd : l__BoolExp  ->  Prims.unit = (fun ( x  :  l__BoolExp ) -> ())
+
+
+let commutativityAnd : l__BoolExp  ->  l__BoolExp  ->  Prims.unit = (fun ( x  :  l__BoolExp ) ( y  :  l__BoolExp ) -> ())
+
+
+let commutativityXor : l__BoolExp  ->  l__BoolExp  ->  Prims.unit = (fun ( x  :  l__BoolExp ) ( y  :  l__BoolExp ) -> ())
+
+
+let distributivityAndXor : l__BoolExp  ->  l__BoolExp  ->  l__BoolExp  ->  Prims.unit = (fun ( x  :  l__BoolExp ) ( y  :  l__BoolExp ) ( z  :  l__BoolExp ) -> ())
+
+
+let rec distribute_preserves_semantics : l__BoolExp  ->  Prims.unit = (fun ( exp  :  l__BoolExp ) -> ())
+
+
+let rec undistribute_preserves_semantics : l__BoolExp  ->  Prims.unit = (fun ( exp  :  l__BoolExp ) -> ())
+
+
+type partition =
+Prims.unit  ->  obj Util.set  ->  obj Util.set  ->  obj Util.set  ->  (((obj, Prims.unit, Prims.unit) Util.disjoint, (obj, Prims.unit, Prims.unit) Util.disjoint) Prims.l_and, (obj, Prims.unit, Prims.unit) Util.disjoint) Prims.l_and
+
+
+let rec compile_decreases_heap : AncillaHeap.l__AncHeap  ->  Prims.int  ->  l__BoolExp  ->  Prims.unit = (fun ( ah  :  AncillaHeap.l__AncHeap ) ( targ  :  Prims.int ) ( exp  :  l__BoolExp ) -> ())
+and compile_decreases_heap_oop : AncillaHeap.l__AncHeap  ->  l__BoolExp  ->  Prims.unit = (fun ( ah  :  AncillaHeap.l__AncHeap ) ( exp  :  l__BoolExp ) -> ())
+
+
+let rec compileClean_decreases_heap : AncillaHeap.l__AncHeap  ->  Prims.int  ->  l__BoolExp  ->  Prims.unit = (fun ( ah  :  AncillaHeap.l__AncHeap ) ( targ  :  Prims.int ) ( exp  :  l__BoolExp ) -> ())
+and compileClean_decreases_heap_oop : AncillaHeap.l__AncHeap  ->  l__BoolExp  ->  Prims.unit = (fun ( ah  :  AncillaHeap.l__AncHeap ) ( exp  :  l__BoolExp ) -> ())
+
+
+let compile_output : AncillaHeap.l__AncHeap  ->  Prims.int  ->  l__BoolExp  ->  Prims.unit = (fun ( ah  :  AncillaHeap.l__AncHeap ) ( targ  :  Prims.int ) ( x  :  l__BoolExp ) -> ())
+
+
+let compile_output_oop : AncillaHeap.l__AncHeap  ->  l__BoolExp  ->  Prims.unit = (fun ( ah  :  AncillaHeap.l__AncHeap ) ( x  :  l__BoolExp ) -> ())
+
+
+let rec compile_partition : AncillaHeap.l__AncHeap  ->  Prims.int  ->  l__BoolExp  ->  Prims.unit = (fun ( ah  :  AncillaHeap.l__AncHeap ) ( targ  :  Prims.int ) ( x  :  l__BoolExp ) -> ())
+and compile_partition_oop : AncillaHeap.l__AncHeap  ->  l__BoolExp  ->  Prims.unit = (fun ( ah  :  AncillaHeap.l__AncHeap ) ( x  :  l__BoolExp ) -> ())
+
+
+let rec compile_mods : AncillaHeap.l__AncHeap  ->  Prims.int  ->  l__BoolExp  ->  Prims.unit = (fun ( ah  :  AncillaHeap.l__AncHeap ) ( targ  :  Prims.int ) ( exp  :  l__BoolExp ) -> ())
+and compile_mods_oop : AncillaHeap.l__AncHeap  ->  l__BoolExp  ->  Prims.unit = (fun ( ah  :  AncillaHeap.l__AncHeap ) ( x  :  l__BoolExp ) -> ())
+
+
+let rec eval_state_swap : l__BoolExp  ->  Total.state  ->  Total.state  ->  Prims.unit = (fun ( x  :  l__BoolExp ) ( st  :  Total.state ) ( st'  :  Total.state ) -> ())
+
+
+let zeroHeap_st_impl : Total.state  ->  AncillaHeap.l__AncHeap  ->  Circuit.l__Gate Prims.list  ->  Prims.unit = (fun ( st  :  Total.state ) ( ah  :  AncillaHeap.l__AncHeap ) ( gates  :  Circuit.l__Gate Prims.list ) -> ())
+
+
+let rec compile_bexp_correct : AncillaHeap.l__AncHeap  ->  Prims.int  ->  l__BoolExp  ->  Total.state  ->  Prims.unit = (fun ( ah  :  AncillaHeap.l__AncHeap ) ( targ  :  Prims.int ) ( exp  :  l__BoolExp ) ( st  :  Total.state ) -> ())
+and compile_bexp_correct_oop : AncillaHeap.l__AncHeap  ->  l__BoolExp  ->  Total.state  ->  Prims.unit = (fun ( ah  :  AncillaHeap.l__AncHeap ) ( exp  :  l__BoolExp ) ( st  :  Total.state ) -> ())
+
+
+let rec compileBexp_wf : AncillaHeap.l__AncHeap  ->  Prims.int  ->  l__BoolExp  ->  Prims.unit = (fun ( ah  :  AncillaHeap.l__AncHeap ) ( targ  :  Prims.int ) ( exp  :  l__BoolExp ) -> ())
+and compileBexp_wf_oop : AncillaHeap.l__AncHeap  ->  l__BoolExp  ->  Prims.unit = (fun ( ah  :  AncillaHeap.l__AncHeap ) ( exp  :  l__BoolExp ) -> ())
+
+
+let rec compile_anc : AncillaHeap.l__AncHeap  ->  Prims.int  ->  l__BoolExp  ->  Prims.unit = (fun ( ah  :  AncillaHeap.l__AncHeap ) ( targ  :  Prims.int ) ( exp  :  l__BoolExp ) -> ())
+and compile_anc_oop : AncillaHeap.l__AncHeap  ->  l__BoolExp  ->  Prims.unit = (fun ( ah  :  AncillaHeap.l__AncHeap ) ( exp  :  l__BoolExp ) -> ())
+
+
+let rec compile_ctrls : AncillaHeap.l__AncHeap  ->  Prims.int  ->  l__BoolExp  ->  Prims.unit = (fun ( ah  :  AncillaHeap.l__AncHeap ) ( targ  :  Prims.int ) ( x  :  l__BoolExp ) -> ())
+and compile_ctrls_oop : AncillaHeap.l__AncHeap  ->  l__BoolExp  ->  Prims.unit = (fun ( ah  :  AncillaHeap.l__AncHeap ) ( x  :  l__BoolExp ) -> ())
+
+
+type ('Aah, 'Atarg, 'Aexp, 'Ast) clean_heap_cond =
+(Prims.unit, Prims.unit) AncillaHeap.zeroHeap
+
+
+type ('Aah, 'Atarg, 'Aexp, 'Ast) clean_corr_cond =
+Prims.unit Prims.b2t
+
+
+let compile_with_cleanup : AncillaHeap.l__AncHeap  ->  Prims.int  ->  l__BoolExp  ->  Total.state  ->  Prims.unit = (fun ( ah  :  AncillaHeap.l__AncHeap ) ( targ  :  Prims.int ) ( exp  :  l__BoolExp ) ( st  :  Total.state ) -> ())
+
+
+let compile_with_cleanup_oop : AncillaHeap.l__AncHeap  ->  l__BoolExp  ->  Total.state  ->  Prims.unit = (fun ( ah  :  AncillaHeap.l__AncHeap ) ( exp  :  l__BoolExp ) ( st  :  Total.state ) -> ())
+
+
+
+
