src/fs/Circuit.fs
@@ -1,0 +1,266 @@
+#light "off"
+module Circuit
+open Prims
+
+type l__Gate =
+| RCNOT of (Prims.int * Prims.int)
+| RTOFF of (Prims.int * Prims.int * Prims.int)
+| RNOT of Prims.int
+
+
+let is_RCNOT = (fun ( _discr_  :  obj ) -> (match (_discr_) with
+| RCNOT (_) -> begin
+true
+end
+| _ -> begin
+false
+end))
+
+
+let is_RTOFF = (fun ( _discr_  :  obj ) -> (match (_discr_) with
+| RTOFF (_) -> begin
+true
+end
+| _ -> begin
+false
+end))
+
+
+let is_RNOT = (fun ( _discr_  :  obj ) -> (match (_discr_) with
+| RNOT (_) -> begin
+true
+end
+| _ -> begin
+false
+end))
+
+
+let ___RCNOT____0 = (fun ( projectee  :  l__Gate ) -> (match (projectee) with
+| RCNOT (_15_3) -> begin
+_15_3
+end))
+
+
+let ___RTOFF____0 = (fun ( projectee  :  l__Gate ) -> (match (projectee) with
+| RTOFF (_15_6) -> begin
+_15_6
+end))
+
+
+let ___RNOT____0 = (fun ( projectee  :  l__Gate ) -> (match (projectee) with
+| RNOT (_15_9) -> begin
+_15_9
+end))
+
+
+type l__Circuit =
+{gates : l__Gate Prims.list; inputs : (Prims.string * Prims.int) Prims.list; outputs : Prims.int Prims.list; ancilla : Prims.int}
+
+
+let is_MkCircuit : l__Circuit  ->  Prims.bool = (Prims.checked_cast(fun ( _  :  l__Circuit ) -> (FStar.All.failwith "Not yet implemented:is_MkCircuit")))
+
+
+let prettyPrintGate : l__Gate  ->  Prims.string = (fun ( gate  :  l__Gate ) -> (match (gate) with
+| RCNOT (a, b) -> begin
+(FStar.String.strcat "tof " (FStar.String.strcat (Prims.string_of_int a) (FStar.String.strcat " " (Prims.string_of_int b))))
+end
+| RTOFF (a, b, c) -> begin
+(FStar.String.strcat "tof " (FStar.String.strcat (Prims.string_of_int a) (FStar.String.strcat " " (FStar.String.strcat (Prims.string_of_int b) (FStar.String.strcat " " (Prims.string_of_int c))))))
+end
+| RNOT (a) -> begin
+(FStar.String.strcat "tof " (Prims.string_of_int a))
+end))
+
+
+let prettyPrintCircuit : l__Gate Prims.list  ->  Prims.string Prims.list = (FStar.List.map prettyPrintGate)
+
+
+let applyGate : Total.state  ->  l__Gate  ->  Total.state = (fun ( st  :  Total.state ) ( gate  :  l__Gate ) -> (match (gate) with
+| RCNOT (a, b) -> begin
+(Total.update st b ((st a) <> (st b)))
+end
+| RTOFF (a, b, c) -> begin
+(Total.update st c ((st c) <> ((st a) && (st b))))
+end
+| RNOT (a) -> begin
+(Total.update st a (not ((st a))))
+end))
+
+
+let rec evalCirc : l__Gate Prims.list  ->  Total.state  ->  Total.state = (fun ( gates  :  l__Gate Prims.list ) ( st  :  Total.state ) -> (match (gates) with
+| [] -> begin
+st
+end
+| x::xs -> begin
+(evalCirc xs (applyGate st x))
+end))
+
+
+let wfGate : l__Gate  ->  Prims.bool = (fun ( gate  :  l__Gate ) -> (match (gate) with
+| RCNOT (a, b) -> begin
+(not ((a = b)))
+end
+| RTOFF (a, b, c) -> begin
+((not ((a = c))) && (not ((b = c))))
+end
+| RNOT (a) -> begin
+true
+end))
+
+
+let rec wfCirc : l__Gate Prims.list  ->  Prims.bool = (fun ( circ  :  l__Gate Prims.list ) -> (match (circ) with
+| [] -> begin
+true
+end
+| x::xs -> begin
+((wfGate x) && (wfCirc xs))
+end))
+
+
+let rec use : Prims.int  ->  l__Gate Prims.list  ->  Prims.bool = (fun ( i  :  Prims.int ) ( lst  :  l__Gate Prims.list ) -> (match (lst) with
+| [] -> begin
+false
+end
+| RCNOT (a, b)::xs -> begin
+(((a = i) || (b = i)) || (use i xs))
+end
+| RTOFF (a, b, c)::xs -> begin
+((((a = i) || (b = i)) || (c = i)) || (use i xs))
+end
+| RNOT (a)::xs -> begin
+((a = i) || (use i xs))
+end))
+
+
+let uses : l__Gate Prims.list  ->  Prims.int Util.set = (fun ( lst  :  l__Gate Prims.list ) ( i  :  Prims.int ) -> (use i lst))
+
+
+let rec mod : Prims.int  ->  l__Gate Prims.list  ->  Prims.bool = (fun ( i  :  Prims.int ) ( gates  :  l__Gate Prims.list ) -> (match (gates) with
+| [] -> begin
+false
+end
+| (RCNOT (_, t)::xs) | (RTOFF (_, _, t)::xs) | (RNOT (t)::xs) -> begin
+((i = t) || (mod i xs))
+end))
+
+
+let mods : l__Gate Prims.list  ->  Prims.int Util.set = (fun ( gates  :  l__Gate Prims.list ) ( i  :  Prims.int ) -> (mod i gates))
+
+
+let rec ctrl : Prims.int  ->  l__Gate Prims.list  ->  Prims.bool = (fun ( i  :  Prims.int ) ( lst  :  l__Gate Prims.list ) -> (match (lst) with
+| [] -> begin
+false
+end
+| RCNOT (a, b)::xs -> begin
+((a = i) || (ctrl i xs))
+end
+| RTOFF (a, b, c)::xs -> begin
+(((a = i) || (b = i)) || (ctrl i xs))
+end
+| RNOT (a)::xs -> begin
+(ctrl i xs)
+end))
+
+
+let ctrls : l__Gate Prims.list  ->  Prims.int Util.set = (fun ( gates  :  l__Gate Prims.list ) ( i  :  Prims.int ) -> (ctrl i gates))
+
+
+let rec uncompute : l__Gate Prims.list  ->  Prims.int  ->  l__Gate Prims.list = (fun ( circ  :  l__Gate Prims.list ) ( targ  :  Prims.int ) -> (match (circ) with
+| [] -> begin
+[]
+end
+| x::xs -> begin
+if (use targ ((x)::[])) then begin
+(uncompute xs targ)
+end else begin
+(x)::(uncompute xs targ)
+end
+end))
+
+
+let rec ref_imp_use : l__Gate Prims.list  ->  Prims.unit = (fun ( gates  :  l__Gate Prims.list ) -> ())
+
+
+let mods_sub_uses : l__Gate Prims.list  ->  Prims.unit = (fun ( gates  :  l__Gate Prims.list ) -> ())
+
+
+let ctrls_sub_uses : l__Gate Prims.list  ->  Prims.unit = (fun ( gates  :  l__Gate Prims.list ) -> ())
+
+
+let apply_mod : Total.state  ->  l__Gate  ->  Prims.unit = (fun ( st  :  Total.state ) ( x  :  l__Gate ) -> ())
+
+
+let rec eval_mod : Total.state  ->  l__Gate Prims.list  ->  Prims.unit = (fun ( st  :  Total.state ) ( gates  :  l__Gate Prims.list ) -> ())
+
+
+let rec evalCirc_append : l__Gate Prims.list  ->  l__Gate Prims.list  ->  Total.state  ->  Prims.unit = (fun ( l1  :  l__Gate Prims.list ) ( l2  :  l__Gate Prims.list ) ( st  :  Total.state ) -> ())
+
+
+let rec use_append : Prims.int  ->  l__Gate Prims.list  ->  l__Gate Prims.list  ->  Prims.unit = (fun ( i  :  Prims.int ) ( x  :  l__Gate Prims.list ) ( y  :  l__Gate Prims.list ) -> ())
+
+
+let rec uses_append : l__Gate Prims.list  ->  l__Gate Prims.list  ->  Prims.unit = (fun ( x  :  l__Gate Prims.list ) ( y  :  l__Gate Prims.list ) -> ())
+
+
+let rec mod_append : Prims.int  ->  l__Gate Prims.list  ->  l__Gate Prims.list  ->  Prims.unit = (fun ( i  :  Prims.int ) ( l1  :  l__Gate Prims.list ) ( l2  :  l__Gate Prims.list ) -> ())
+
+
+let rec mods_append : l__Gate Prims.list  ->  l__Gate Prims.list  ->  Prims.unit = (fun ( x  :  l__Gate Prims.list ) ( y  :  l__Gate Prims.list ) -> ())
+
+
+let rec ctrl_append : Prims.int  ->  l__Gate Prims.list  ->  l__Gate Prims.list  ->  Prims.unit = (fun ( i  :  Prims.int ) ( x  :  l__Gate Prims.list ) ( y  :  l__Gate Prims.list ) -> ())
+
+
+let rec ctrls_append : l__Gate Prims.list  ->  l__Gate Prims.list  ->  Prims.unit = (fun ( x  :  l__Gate Prims.list ) ( y  :  l__Gate Prims.list ) -> ())
+
+
+let rec wf_append : l__Gate Prims.list  ->  l__Gate Prims.list  ->  Prims.unit = (fun ( x  :  l__Gate Prims.list ) ( y  :  l__Gate Prims.list ) -> ())
+
+
+let rec rev_uses : l__Gate Prims.list  ->  Prims.unit = (fun ( circ  :  l__Gate Prims.list ) -> ())
+
+
+let rec rev_mods : l__Gate Prims.list  ->  Prims.unit = (fun ( circ  :  l__Gate Prims.list ) -> ())
+
+
+let rec rev_ctrls : l__Gate Prims.list  ->  Prims.unit = (fun ( circ  :  l__Gate Prims.list ) -> ())
+
+
+let evalCirc_append_rev : l__Gate Prims.list  ->  l__Gate Prims.list  ->  Total.state  ->  Prims.unit = (fun ( x  :  l__Gate Prims.list ) ( y  :  l__Gate Prims.list ) ( st  :  Total.state ) -> ())
+
+
+let rev_gate : l__Gate  ->  Total.state  ->  Prims.unit = (fun ( gate  :  l__Gate ) ( st  :  Total.state ) -> ())
+
+
+let rec rev_inverse : l__Gate Prims.list  ->  Total.state  ->  Prims.unit = (fun ( circ  :  l__Gate Prims.list ) ( st  :  Total.state ) -> ())
+
+
+let applyGate_state_swap : l__Gate  ->  Total.state  ->  Total.state  ->  Prims.int Util.set  ->  Prims.unit = (fun ( x  :  l__Gate ) ( st  :  Total.state ) ( st'  :  Total.state ) ( dom  :  Prims.int Util.set ) -> ())
+
+
+let rec evalCirc_state_swap : l__Gate Prims.list  ->  Total.state  ->  Total.state  ->  Prims.int Util.set  ->  Prims.unit = (fun ( circ  :  l__Gate Prims.list ) ( st  :  Total.state ) ( st'  :  Total.state ) ( dom  :  Prims.int Util.set ) -> ())
+
+
+let bennett : l__Gate Prims.list  ->  l__Gate Prims.list  ->  Total.state  ->  Prims.unit = (fun ( comp  :  l__Gate Prims.list ) ( copy  :  l__Gate Prims.list ) ( st  :  Total.state ) -> ())
+
+
+let rec uncompute_targ : l__Gate Prims.list  ->  Prims.int  ->  Prims.unit = (fun ( circ  :  l__Gate Prims.list ) ( targ  :  Prims.int ) -> ())
+
+
+let rec uncompute_wf : l__Gate Prims.list  ->  Prims.int  ->  Prims.unit = (fun ( circ  :  l__Gate Prims.list ) ( targ  :  Prims.int ) -> ())
+
+
+let rec uncompute_uses_subset : l__Gate Prims.list  ->  Prims.int  ->  Prims.unit = (fun ( circ  :  l__Gate Prims.list ) ( targ  :  Prims.int ) -> ())
+
+
+let rec uncompute_ctrls_subset : l__Gate Prims.list  ->  Prims.int  ->  Prims.unit = (fun ( circ  :  l__Gate Prims.list ) ( targ  :  Prims.int ) -> ())
+
+
+let rec uncompute_agree : l__Gate Prims.list  ->  Prims.int  ->  Total.state  ->  Prims.unit = (fun ( circ  :  l__Gate Prims.list ) ( targ  :  Prims.int ) ( st  :  Total.state ) -> ())
+
+
+let uncompute_mixed_inverse : l__Gate Prims.list  ->  Prims.int  ->  Total.state  ->  Prims.unit = (fun ( circ  :  l__Gate Prims.list ) ( targ  :  Prims.int ) ( st  :  Total.state ) -> ())
+
+
+
+
