src/fs/FStar.All.fs
@@ -1,0 +1,27 @@
+#light "off"
+module FStar.All
+open Prims
+
+let pipe_right = (fun ( _  :  'a ) ( _  :  'a  ->  'b ) -> (failwith "Not yet implemented:pipe_right"))
+
+
+let pipe_left = (fun ( _  :  'a  ->  'b ) ( _  :  'a ) -> (failwith "Not yet implemented:pipe_left"))
+
+
+let failwith = (fun ( _  :  Prims.string ) -> (failwith "Not yet implemented:failwith"))
+
+
+let exit = (fun ( _  :  Prims.int ) -> (failwith "Not yet implemented:exit"))
+
+
+let try_with = (fun ( _  :  Prims.unit  ->  'a ) ( _  :  Prims.exn  ->  'a ) -> (failwith "Not yet implemented:try_with"))
+
+
+let op_Less_Less = (fun ( _  :  'b  ->  'c ) ( _  :  'a  ->  'b ) ( _  :  'a ) -> (failwith "Not yet implemented:op_Less_Less"))
+
+
+let op_Greater_Greater = (fun ( _  :  'a  ->  'b ) ( _  :  'b  ->  'c ) ( _  :  'a ) -> (failwith "Not yet implemented:op_Greater_Greater"))
+
+
+
+
