src/fs/FStar.FunctionalExtensionality.fs
@@ -1,0 +1,10 @@
+#light "off"
+module FStar.FunctionalExtensionality
+open Prims
+
+type ('Aa, 'Ab) efun =
+'Aa  ->  'Ab
+
+
+
+
