src/fs/FStar.ST.fs
@@ -1,0 +1,28 @@
+#light "off"
+module FStar.ST
+open Prims
+
+type 'Aa ref =
+'Aa FStar.Heap.ref
+
+
+let recall = (fun ( r  :  'Aa ref ) -> (FStar.All.failwith "Not yet implemented:recall"))
+
+
+let alloc = (fun ( init  :  'Aa ) -> (FStar.All.failwith "Not yet implemented:alloc"))
+
+
+let read = (fun ( r  :  'Aa ref ) -> (FStar.All.failwith "Not yet implemented:read"))
+
+
+let write = (fun ( r  :  'Aa ref ) ( v  :  'Aa ) -> (FStar.All.failwith "Not yet implemented:write"))
+
+
+let op_Colon_Equals = (fun ( r  :  'Aa ref ) ( v  :  'Aa ) -> (FStar.All.failwith "Not yet implemented:op_Colon_Equals"))
+
+
+let get : Prims.unit  ->  FStar.Heap.heap = (fun ( _  :  Prims.unit ) -> (FStar.All.failwith "Not yet implemented:get"))
+
+
+
+
