src/fs/Interpreter.fs
@@ -1,0 +1,1052 @@
+#light "off"
+module Interpreter
+open Prims
+
+type 'Astate interpretation =
+{alloc : 'Astate  ->  BoolExp.l__BoolExp  ->  (Prims.int * 'Astate); assign : 'Astate  ->  Prims.int  ->  BoolExp.l__BoolExp  ->  'Astate; eval : 'Astate  ->  Total.state  ->  Prims.int  ->  Prims.bool}
+
+
+let is_Mkinterpretation = (Prims.checked_cast(fun ( _  :  'Astate interpretation ) -> (FStar.All.failwith "Not yet implemented:is_Mkinterpretation")))
+
+
+let rec isVal : ExprTypes.l__GExpr  ->  Prims.bool = (fun ( tm  :  ExprTypes.l__GExpr ) -> (match (tm) with
+| ExprTypes.UNIT -> begin
+true
+end
+| ExprTypes.LAMBDA (s, ty, t) -> begin
+true
+end
+| ExprTypes.LOC (i) -> begin
+true
+end
+| ExprTypes.ARRAY (lst) -> begin
+(isVal_lst lst)
+end
+| _18_20 -> begin
+false
+end))
+and isVal_lst : ExprTypes.l__GExpr Prims.list  ->  Prims.bool = (fun ( lst  :  ExprTypes.l__GExpr Prims.list ) -> (match (lst) with
+| [] -> begin
+true
+end
+| ExprTypes.LOC (l)::xs -> begin
+(isVal_lst xs)
+end
+| _18_28 -> begin
+false
+end))
+
+
+let isBexp : ExprTypes.l__GExpr  ->  Prims.bool = (fun ( tm  :  ExprTypes.l__GExpr ) -> (match (tm) with
+| ExprTypes.LOC (i) -> begin
+true
+end
+| ExprTypes.BEXP (bexp) -> begin
+true
+end
+| ExprTypes.BOOL (b) -> begin
+true
+end
+| _18_37 -> begin
+false
+end))
+
+
+type 'Astate config =
+(ExprTypes.l__GExpr * 'Astate)
+
+
+type 'Astate valconfig =
+'Astate config
+
+
+type 'Astate listconfig =
+(ExprTypes.l__GExpr Prims.list * 'Astate)
+
+
+let get_bexp : ExprTypes.l__GExpr  ->  BoolExp.l__BoolExp = (fun ( gexp  :  ExprTypes.l__GExpr ) -> (match (gexp) with
+| ExprTypes.LOC (i) -> begin
+BoolExp.BVar (i)
+end
+| ExprTypes.BEXP (bexp) -> begin
+bexp
+end
+| ExprTypes.BOOL (b) -> begin
+if b then begin
+BoolExp.BNot (BoolExp.BFalse)
+end else begin
+BoolExp.BFalse
+end
+end))
+
+
+let rec step = (fun ( _18_57  :  'Astate config ) ( interp  :  'Astate interpretation ) -> (match (_18_57) with
+| (tm, st) -> begin
+(match (tm) with
+| ExprTypes.LET (x, t1, t2) -> begin
+if (isVal t1) then begin
+Util.Val (((ExprTypes.substGExpr t2 x t1), st))
+end else begin
+(Util.bindT (step (t1, st) interp) (fun ( _18_66  :  'Astate config ) -> (match (_18_66) with
+| (t1', st') -> begin
+Util.Val ((ExprTypes.LET ((x, t1', t2)), st'))
+end)))
+end
+end
+| ExprTypes.APPLY (t1, t2) -> begin
+if (not ((isVal t1))) then begin
+(Util.bindT (step (t1, st) interp) (fun ( _18_73  :  'Astate config ) -> (match (_18_73) with
+| (t1', st') -> begin
+Util.Val ((ExprTypes.APPLY ((t1', t2)), st'))
+end)))
+end else begin
+if (not ((isVal t2))) then begin
+(Util.bindT (step (t2, st) interp) (fun ( _18_76  :  'Astate config ) -> (match (_18_76) with
+| (t2', st') -> begin
+Util.Val ((ExprTypes.APPLY ((t1, t2')), st'))
+end)))
+end else begin
+(match (t1) with
+| ExprTypes.LAMBDA (x, ty, t) -> begin
+Util.Val (((ExprTypes.substGExpr t x t2), st))
+end
+| _18_83 -> begin
+Util.Err ((FStar.String.strcat "Cannot reduce application: " (ExprTypes.show tm)))
+end)
+end
+end
+end
+| ExprTypes.SEQUENCE (t1, t2) -> begin
+if (not ((isVal t1))) then begin
+(Util.bindT (step (t1, st) interp) (fun ( _18_90  :  'Astate config ) -> (match (_18_90) with
+| (t1', st') -> begin
+Util.Val ((ExprTypes.SEQUENCE ((t1', t2)), st'))
+end)))
+end else begin
+(match (t1) with
+| ExprTypes.UNIT -> begin
+Util.Val ((t2, st))
+end
+| _18_93 -> begin
+Util.Err ((FStar.String.strcat "Cannot reduce sequence: " (ExprTypes.show tm)))
+end)
+end
+end
+| ExprTypes.ASSIGN (t1, t2) -> begin
+if (not ((isVal t1))) then begin
+(Util.bindT (step (t1, st) interp) (fun ( _18_100  :  'Astate config ) -> (match (_18_100) with
+| (t1', st') -> begin
+Util.Val ((ExprTypes.ASSIGN ((t1', t2)), st'))
+end)))
+end else begin
+if (not ((isBexp t2))) then begin
+(Util.bindT (step (t2, st) interp) (fun ( _18_103  :  'Astate config ) -> (match (_18_103) with
+| (t2', st') -> begin
+Util.Val ((ExprTypes.ASSIGN ((t1, t2')), st'))
+end)))
+end else begin
+(match (t1) with
+| ExprTypes.LOC (l) -> begin
+Util.Val ((ExprTypes.UNIT, (interp.assign st l (get_bexp t2))))
+end
+| _18_107 -> begin
+Util.Err ((FStar.String.strcat "Cannot reduce assignment: " (ExprTypes.show tm)))
+end)
+end
+end
+end
+| ExprTypes.XOR (t1, t2) -> begin
+if (not ((isBexp t1))) then begin
+(Util.bindT (step (t1, st) interp) (fun ( _18_114  :  'Astate config ) -> (match (_18_114) with
+| (t1', st') -> begin
+Util.Val ((ExprTypes.XOR ((t1', t2)), st'))
+end)))
+end else begin
+if (not ((isBexp t2))) then begin
+(Util.bindT (step (t2, st) interp) (fun ( _18_117  :  'Astate config ) -> (match (_18_117) with
+| (t2', st') -> begin
+Util.Val ((ExprTypes.XOR ((t1, t2')), st'))
+end)))
+end else begin
+Util.Val ((ExprTypes.BEXP (BoolExp.BXor (((get_bexp t1), (get_bexp t2)))), st))
+end
+end
+end
+| ExprTypes.AND (t1, t2) -> begin
+if (not ((isBexp t1))) then begin
+(Util.bindT (step (t1, st) interp) (fun ( _18_124  :  'Astate config ) -> (match (_18_124) with
+| (t1', st') -> begin
+Util.Val ((ExprTypes.AND ((t1', t2)), st'))
+end)))
+end else begin
+if (not ((isBexp t2))) then begin
+(Util.bindT (step (t2, st) interp) (fun ( _18_127  :  'Astate config ) -> (match (_18_127) with
+| (t2', st') -> begin
+Util.Val ((ExprTypes.AND ((t1, t2')), st'))
+end)))
+end else begin
+Util.Val ((ExprTypes.BEXP (BoolExp.BAnd (((get_bexp t1), (get_bexp t2)))), st))
+end
+end
+end
+| ExprTypes.BOOL (b) -> begin
+(
+
+let bexp = if b then begin
+BoolExp.BNot (BoolExp.BFalse)
+end else begin
+BoolExp.BFalse
+end
+in Util.Val ((ExprTypes.BEXP (bexp), st)))
+end
+| ExprTypes.APPEND (t1, t2) -> begin
+if (not ((isVal t1))) then begin
+(Util.bindT (step (t1, st) interp) (fun ( _18_137  :  'Astate config ) -> (match (_18_137) with
+| (t1', st') -> begin
+Util.Val ((ExprTypes.APPLY ((t1', t2)), st'))
+end)))
+end else begin
+if (not ((isVal t2))) then begin
+(Util.bindT (step (t2, st) interp) (fun ( _18_140  :  'Astate config ) -> (match (_18_140) with
+| (t2', st') -> begin
+Util.Val ((ExprTypes.APPLY ((t1, t2')), st'))
+end)))
+end else begin
+(match ((t1, t2)) with
+| (ExprTypes.ARRAY (l), ExprTypes.ARRAY (l')) -> begin
+Util.Val ((ExprTypes.ARRAY ((FStar.List.append l l')), st))
+end
+| _18_147 -> begin
+Util.Err ((FStar.String.strcat "Cannot reduce append: " (ExprTypes.show tm)))
+end)
+end
+end
+end
+| ExprTypes.ROT (i, t) -> begin
+if (not ((isVal t))) then begin
+(Util.bindT (step (t, st) interp) (fun ( _18_154  :  'Astate config ) -> (match (_18_154) with
+| (t', st') -> begin
+Util.Val ((ExprTypes.ROT ((i, t')), st'))
+end)))
+end else begin
+(match (t) with
+| ExprTypes.ARRAY (lst) -> begin
+if ((0 <= i) && (i < (FStar.List.lengthT lst))) then begin
+Util.Val ((ExprTypes.ARRAY ((Util.rotate lst i)), st))
+end else begin
+Util.Err ((FStar.String.strcat "Array out of bounds: " (ExprTypes.show tm)))
+end
+end
+| _18_158 -> begin
+Util.Err ((FStar.String.strcat "Cannot reduce rotation: " (ExprTypes.show tm)))
+end)
+end
+end
+| ExprTypes.SLICE (t, i, j) -> begin
+if (not ((isVal t))) then begin
+(Util.bindT (step (t, st) interp) (fun ( _18_166  :  'Astate config ) -> (match (_18_166) with
+| (t', st') -> begin
+Util.Val ((ExprTypes.SLICE ((t', i, j)), st'))
+end)))
+end else begin
+(match (t) with
+| ExprTypes.ARRAY (lst) -> begin
+if (((0 <= i) && (i <= j)) && (j < (FStar.List.lengthT lst))) then begin
+Util.Val ((ExprTypes.ARRAY ((Util.slice lst i j)), st))
+end else begin
+Util.Err ((FStar.String.strcat "Array out of bounds: " (ExprTypes.show tm)))
+end
+end
+| _18_170 -> begin
+Util.Err ((FStar.String.strcat "Cannot reduce slice: " (ExprTypes.show tm)))
+end)
+end
+end
+| ExprTypes.ARRAY (lst) -> begin
+(Util.bindT (step_lst (lst, st) interp) (fun ( _18_175  :  'Astate listconfig ) -> (match (_18_175) with
+| (lst, st') -> begin
+Util.Val ((ExprTypes.ARRAY (lst), st'))
+end)))
+end
+| ExprTypes.GET_ARRAY (t, i) -> begin
+if (not ((isVal t))) then begin
+(Util.bindT (step (t, st) interp) (fun ( _18_182  :  'Astate config ) -> (match (_18_182) with
+| (t', st') -> begin
+Util.Val ((ExprTypes.GET_ARRAY ((t', i)), st'))
+end)))
+end else begin
+(match (t) with
+| ExprTypes.ARRAY (lst) -> begin
+if ((0 <= i) && (i < (FStar.List.lengthT lst))) then begin
+Util.Val (((Util.nthT lst i), st))
+end else begin
+Util.Err ((FStar.String.strcat "Array out of bounds: " (ExprTypes.show tm)))
+end
+end
+| _18_186 -> begin
+Util.Err ((FStar.String.strcat "Cannot reduce array index: " (ExprTypes.show tm)))
+end)
+end
+end
+| ExprTypes.ASSERT (t) -> begin
+if (not ((isVal t))) then begin
+(Util.bindT (step (t, st) interp) (fun ( _18_191  :  'Astate config ) -> (match (_18_191) with
+| (t', st') -> begin
+Util.Val ((ExprTypes.ASSERT (t'), st'))
+end)))
+end else begin
+(match (t) with
+| ExprTypes.LOC (l) -> begin
+Util.Val ((ExprTypes.UNIT, st))
+end
+| _18_195 -> begin
+Util.Err ((FStar.String.strcat "Cannot reduce assertion: " (ExprTypes.show tm)))
+end)
+end
+end
+| ExprTypes.BEXP (bexp) -> begin
+(
+
+let _18_200 = (interp.alloc st bexp)
+in (match (_18_200) with
+| (l, st') -> begin
+Util.Val ((ExprTypes.LOC (l), st'))
+end))
+end
+| _18_202 -> begin
+Util.Err ((FStar.String.strcat "No rule applies: " (ExprTypes.show tm)))
+end)
+end))
+and step_lst = (fun ( _18_205  :  'Astate listconfig ) ( interp  :  'Astate interpretation ) -> (match (_18_205) with
+| (lst, st) -> begin
+(match (lst) with
+| [] -> begin
+Util.Val (([], st))
+end
+| x::xs -> begin
+if (not ((isVal x))) then begin
+(Util.bindT (step (x, st) interp) (fun ( _18_213  :  'Astate config ) -> (match (_18_213) with
+| (x', st') -> begin
+Util.Val (((x')::xs, st'))
+end)))
+end else begin
+(Util.bindT (step_lst (xs, st) interp) (fun ( _18_216  :  'Astate listconfig ) -> (match (_18_216) with
+| (xs', st') -> begin
+Util.Val (((x)::xs', st'))
+end)))
+end
+end)
+end))
+
+
+let rec eval_rec = (fun ( _18_221  :  'Astate config ) ( interp  :  'Astate interpretation ) -> (match (_18_221) with
+| (tm, st) -> begin
+(match (tm) with
+| ExprTypes.LET (x, t1, t2) -> begin
+(Util.bind (eval_rec (t1, st) interp) (fun ( _18_230  :  'Astate config ) -> (match (_18_230) with
+| (v1, st') -> begin
+(eval_rec ((ExprTypes.substGExpr t2 x v1), st') interp)
+end)))
+end
+| ExprTypes.LAMBDA (x, ty, t) -> begin
+Util.Val ((tm, st))
+end
+| ExprTypes.APPLY (t1, t2) -> begin
+(Util.bind (eval_rec (t1, st) interp) (fun ( _18_242  :  'Astate config ) -> (match (_18_242) with
+| (v1, st') -> begin
+(Util.bind (eval_rec (t2, st') interp) (fun ( _18_245  :  'Astate config ) -> (match (_18_245) with
+| (v2, st'') -> begin
+(match (v1) with
+| ExprTypes.LAMBDA (x, ty, t) -> begin
+(eval_rec ((ExprTypes.substGExpr t x v2), st'') interp)
+end
+| _18_252 -> begin
+Util.Err ((FStar.String.strcat "LHS is not a lambda: " (ExprTypes.show tm)))
+end)
+end)))
+end)))
+end
+| ExprTypes.SEQUENCE (t1, t2) -> begin
+(Util.bind (eval_rec (t1, st) interp) (fun ( _18_259  :  'Astate config ) -> (match (_18_259) with
+| (v1, st') -> begin
+(eval_rec (t2, st') interp)
+end)))
+end
+| ExprTypes.ASSIGN (t1, t2) -> begin
+(Util.bind (eval_rec (t1, st) interp) (fun ( _18_266  :  'Astate config ) -> (match (_18_266) with
+| (v1, st') -> begin
+(Util.bind (eval_rec (t2, st') interp) (fun ( _18_269  :  'Astate config ) -> (match (_18_269) with
+| (v2, st'') -> begin
+(match ((v1, v2)) with
+| (ExprTypes.LOC (l), ExprTypes.BEXP (bexp)) -> begin
+Util.Val ((ExprTypes.UNIT, (interp.assign st' l bexp)))
+end
+| _18_276 -> begin
+Util.Err ((FStar.String.strcat "Invalid parameters: " (ExprTypes.show tm)))
+end)
+end)))
+end)))
+end
+| (ExprTypes.XOR (_)) | (ExprTypes.AND (_)) | (ExprTypes.BOOL (_)) -> begin
+(Util.bind (eval_to_bexp (tm, st) interp) (fun ( c  :  'Astate config ) -> (eval_rec c interp)))
+end
+| ExprTypes.APPEND (t1, t2) -> begin
+(Util.bind (eval_rec (t1, st) interp) (fun ( _18_293  :  'Astate config ) -> (match (_18_293) with
+| (v1, st') -> begin
+(Util.bind (eval_rec (t2, st') interp) (fun ( _18_296  :  'Astate config ) -> (match (_18_296) with
+| (v2, st'') -> begin
+(match ((v1, v2)) with
+| (ExprTypes.ARRAY (l1), ExprTypes.ARRAY (l2)) -> begin
+Util.Val ((ExprTypes.ARRAY ((FStar.List.append l1 l2)), st''))
+end
+| _18_303 -> begin
+Util.Err ((FStar.String.strcat "Append of non-array argument: " (ExprTypes.show tm)))
+end)
+end)))
+end)))
+end
+| ExprTypes.ROT (i, t) -> begin
+(Util.bind (eval_rec (t, st) interp) (fun ( _18_310  :  'Astate config ) -> (match (_18_310) with
+| (v, st') -> begin
+(match (v) with
+| ExprTypes.ARRAY (lst) -> begin
+if ((0 <= i) && (i < (FStar.List.length lst))) then begin
+Util.Val ((ExprTypes.ARRAY ((Util.rotate lst i)), st'))
+end else begin
+Util.Err ((FStar.String.strcat "Rotation out of array bounds: " (ExprTypes.show tm)))
+end
+end
+| _18_314 -> begin
+Util.Err ((FStar.String.strcat "Rotation of non-array argument: " (ExprTypes.show tm)))
+end)
+end)))
+end
+| ExprTypes.SLICE (t, i, j) -> begin
+(Util.bind (eval_rec (t, st) interp) (fun ( _18_322  :  'Astate config ) -> (match (_18_322) with
+| (v, st') -> begin
+(match (v) with
+| ExprTypes.ARRAY (lst) -> begin
+if (((0 <= i) && (i <= j)) && (j < (FStar.List.length lst))) then begin
+Util.Val ((ExprTypes.ARRAY ((Util.slice lst i j)), st'))
+end else begin
+Util.Err ((FStar.String.strcat "Invalid slice bounds: " (ExprTypes.show tm)))
+end
+end
+| _18_326 -> begin
+Util.Err ((FStar.String.strcat "Slice of non-array argument: " (ExprTypes.show tm)))
+end)
+end)))
+end
+| ExprTypes.ARRAY (tlst) -> begin
+(
+
+let f = (fun ( _18_332  :  (ExprTypes.l__GExpr Prims.list * 'Astate) ) ( t  :  ExprTypes.l__GExpr ) -> (match (_18_332) with
+| (acc, st) -> begin
+(Util.bind (eval_rec (t, st) interp) (fun ( _18_336  :  'Astate config ) -> (match (_18_336) with
+| (v, st') -> begin
+(match (v) with
+| ExprTypes.LOC (l) -> begin
+Util.Val (((v)::acc, st'))
+end
+| _18_340 -> begin
+Util.Err ((FStar.String.strcat "Array argument not boolean: " (ExprTypes.show t)))
+end)
+end)))
+end))
+in (Util.bind (Util.foldM f ([], st) tlst) (fun ( _18_343  :  (ExprTypes.l__GExpr Prims.list * 'Astate) ) -> (match (_18_343) with
+| (llst, st') -> begin
+Util.Val ((ExprTypes.ARRAY ((FStar.List.rev llst)), st'))
+end))))
+end
+| ExprTypes.GET_ARRAY (t, i) -> begin
+(Util.bind (eval_rec (t, st) interp) (fun ( _18_350  :  'Astate config ) -> (match (_18_350) with
+| (v, st') -> begin
+(match (v) with
+| ExprTypes.ARRAY (lst) -> begin
+if ((0 <= i) && (i < (FStar.List.length lst))) then begin
+(match ((FStar.List.total_nth lst i)) with
+| Some (ExprTypes.LOC (l)) -> begin
+Util.Val ((ExprTypes.LOC (l), st'))
+end
+| Some (_18_357) -> begin
+Util.Err ("Impossible")
+end
+| None -> begin
+Util.Err ((FStar.String.strcat "Array out of bounds: " (ExprTypes.show tm)))
+end)
+end else begin
+Util.Err ((FStar.String.strcat "Array out of bounds: " (ExprTypes.show tm)))
+end
+end
+| _18_361 -> begin
+Util.Err ((FStar.String.strcat "Invalid parameters: " (ExprTypes.show tm)))
+end)
+end)))
+end
+| ExprTypes.VAR (x) -> begin
+Util.Val ((tm, st))
+end
+| ExprTypes.ASSERT (t) -> begin
+(Util.bind (eval_rec (t, st) interp) (fun ( _18_368  :  'Astate config ) -> (match (_18_368) with
+| (v, st') -> begin
+(match (v) with
+| ExprTypes.LOC (l) -> begin
+Util.Val ((ExprTypes.UNIT, st'))
+end
+| _18_372 -> begin
+Util.Err ((FStar.String.strcat "Assert of non-boolean argument: " (ExprTypes.show tm)))
+end)
+end)))
+end
+| ExprTypes.BEXP (bexp) -> begin
+(
+
+let _18_377 = (interp.alloc st bexp)
+in (match (_18_377) with
+| (l, st') -> begin
+Util.Val ((ExprTypes.LOC (l), st'))
+end))
+end
+| _18_379 -> begin
+Util.Err ((FStar.String.strcat "Unimplemented case: " (ExprTypes.show tm)))
+end)
+end))
+and eval_to_bexp = (fun ( _18_382  :  'Astate config ) ( interp  :  'Astate interpretation ) -> (match (_18_382) with
+| (tm, st) -> begin
+(match (tm) with
+| ExprTypes.XOR (x, y) -> begin
+(Util.bind (eval_to_bexp (x, st) interp) (fun ( _18_390  :  'Astate config ) -> (match (_18_390) with
+| (x', st') -> begin
+(Util.bind (eval_to_bexp (y, st') interp) (fun ( _18_393  :  'Astate config ) -> (match (_18_393) with
+| (y', st'') -> begin
+(match ((x', y')) with
+| (ExprTypes.BEXP (b), ExprTypes.BEXP (b')) -> begin
+Util.Val ((ExprTypes.BEXP (BoolExp.BXor ((b, b'))), st''))
+end
+| _18_400 -> begin
+Util.Err ((FStar.String.strcat "Could not reduce parameters to booleans: " (ExprTypes.show tm)))
+end)
+end)))
+end)))
+end
+| ExprTypes.AND (x, y) -> begin
+(Util.bind (eval_to_bexp (x, st) interp) (fun ( _18_407  :  'Astate config ) -> (match (_18_407) with
+| (x', st') -> begin
+(Util.bind (eval_to_bexp (y, st') interp) (fun ( _18_410  :  'Astate config ) -> (match (_18_410) with
+| (y', st'') -> begin
+(match ((x', y')) with
+| (ExprTypes.BEXP (b), ExprTypes.BEXP (b')) -> begin
+Util.Val ((ExprTypes.BEXP (BoolExp.BAnd ((b, b'))), st''))
+end
+| _18_417 -> begin
+Util.Err ((FStar.String.strcat "Could not reduce parameters to booleans: " (ExprTypes.show tm)))
+end)
+end)))
+end)))
+end
+| ExprTypes.BOOL (b) -> begin
+if b then begin
+Util.Val ((ExprTypes.BEXP (BoolExp.BNot (BoolExp.BFalse)), st))
+end else begin
+Util.Val ((ExprTypes.BEXP (BoolExp.BFalse), st))
+end
+end
+| _18_421 -> begin
+(Util.bind (eval_rec (tm, st) interp) (fun ( _18_424  :  'Astate config ) -> (match (_18_424) with
+| (v, st') -> begin
+(match (v) with
+| ExprTypes.LOC (l) -> begin
+Util.Val ((ExprTypes.BEXP (BoolExp.BVar (l)), st'))
+end
+| _18_428 -> begin
+Util.Err ((FStar.String.strcat "Could not reduce expression to boolean: " (ExprTypes.show tm)))
+end)
+end)))
+end)
+end))
+
+
+type boolState =
+(Prims.int * (Prims.int, Prims.bool) Total.map)
+
+
+let boolInit : (Prims.int * (Prims.int  ->  Prims.bool)) = (0, (Total.const false))
+
+
+let boolAlloc : boolState  ->  BoolExp.l__BoolExp  ->  (Prims.int * boolState) = (fun ( _18_431  :  boolState ) ( bexp  :  BoolExp.l__BoolExp ) -> (match (_18_431) with
+| (top, st) -> begin
+(top, ((top + 1), (Total.update st top (BoolExp.evalBexp bexp st))))
+end))
+
+
+let boolAssign : boolState  ->  Prims.int  ->  BoolExp.l__BoolExp  ->  boolState = (fun ( _18_435  :  boolState ) ( l  :  Prims.int ) ( bexp  :  BoolExp.l__BoolExp ) -> (match (_18_435) with
+| (top, st) -> begin
+(top, (Total.update st l (BoolExp.evalBexp bexp st)))
+end))
+
+
+let boolEval : boolState  ->  Total.state  ->  Prims.int  ->  Prims.bool = (fun ( _18_440  :  boolState ) ( ivals  :  Total.state ) ( i  :  Prims.int ) -> (match (_18_440) with
+| (top, st) -> begin
+(Total.lookup st i)
+end))
+
+
+let boolInterp : boolState interpretation = {alloc = boolAlloc; assign = boolAssign; eval = boolEval}
+
+
+let rec substVal : ExprTypes.l__GExpr  ->  boolState  ->  ExprTypes.l__GExpr = (fun ( v  :  ExprTypes.l__GExpr ) ( st  :  boolState ) -> (match (v) with
+| (ExprTypes.UNIT) | (ExprTypes.LAMBDA (_)) -> begin
+v
+end
+| ExprTypes.LOC (l) -> begin
+ExprTypes.BOOL ((Total.lookup (Prims.snd st) l))
+end
+| ExprTypes.ARRAY (lst) -> begin
+ExprTypes.ARRAY ((substVal_lst lst st))
+end))
+and substVal_lst : ExprTypes.l__GExpr Prims.list  ->  boolState  ->  ExprTypes.l__GExpr Prims.list = (fun ( lst  :  ExprTypes.l__GExpr Prims.list ) ( st  :  boolState ) -> (match (lst) with
+| [] -> begin
+[]
+end
+| ExprTypes.LOC (l)::xs -> begin
+(ExprTypes.BOOL ((Total.lookup (Prims.snd st) l)))::(substVal_lst xs st)
+end))
+
+
+let rec evalBool : (ExprTypes.l__GExpr * (Prims.int * (Prims.int  ->  Prims.bool)))  ->  Prims.string Prims.list = (fun ( _18_468  :  (ExprTypes.l__GExpr * (Prims.int * (Prims.int  ->  Prims.bool))) ) -> (match (_18_468) with
+| (gexp, st) -> begin
+if (isVal gexp) then begin
+(ExprTypes.prettyPrint (substVal gexp st))
+end else begin
+(match ((step (gexp, st) boolInterp)) with
+| Util.Err (s) -> begin
+(s)::[]
+end
+| Util.Val (c') -> begin
+(evalBool c')
+end)
+end
+end))
+
+
+let eval : ExprTypes.l__GExpr  ->  Prims.string Prims.list = (fun ( gexp  :  ExprTypes.l__GExpr ) -> (evalBool (gexp, boolInit)))
+
+
+type l__BExpState =
+(Prims.int * (Prims.int, BoolExp.l__BoolExp) Total.map)
+
+
+let bexpInit : (Prims.int * (Prims.int  ->  BoolExp.l__BoolExp)) = (0, (Total.const BoolExp.BFalse))
+
+
+let bexpAlloc : l__BExpState  ->  BoolExp.l__BoolExp  ->  (Prims.int * l__BExpState) = (fun ( _18_476  :  l__BExpState ) ( bexp  :  BoolExp.l__BoolExp ) -> (match (_18_476) with
+| (top, st) -> begin
+(top, ((top + 1), (Total.update st top (BoolExp.substBexp bexp st))))
+end))
+
+
+let bexpAssign : l__BExpState  ->  Prims.int  ->  BoolExp.l__BoolExp  ->  l__BExpState = (fun ( _18_480  :  l__BExpState ) ( l  :  Prims.int ) ( bexp  :  BoolExp.l__BoolExp ) -> (match (_18_480) with
+| (top, st) -> begin
+(top, (Total.update st l (BoolExp.substBexp bexp st)))
+end))
+
+
+let bexpEval : l__BExpState  ->  Total.state  ->  Prims.int  ->  Prims.bool = (fun ( _18_485  :  l__BExpState ) ( ivals  :  Total.state ) ( i  :  Prims.int ) -> (match (_18_485) with
+| (top, st) -> begin
+(BoolExp.evalBexp (Total.lookup st i) ivals)
+end))
+
+
+let bexpInterp : l__BExpState interpretation = {alloc = bexpAlloc; assign = bexpAssign; eval = bexpEval}
+
+
+type l__CleanupStrategy =
+| Pebbled
+| Boundaries
+| Bennett
+
+
+let is_Pebbled = (fun ( _discr_  :  obj ) -> (match (_discr_) with
+| Pebbled (_) -> begin
+true
+end
+| _ -> begin
+false
+end))
+
+
+let is_Boundaries = (fun ( _discr_  :  obj ) -> (match (_discr_) with
+| Boundaries (_) -> begin
+true
+end
+| _ -> begin
+false
+end))
+
+
+let is_Bennett = (fun ( _discr_  :  obj ) -> (match (_discr_) with
+| Bennett (_) -> begin
+true
+end
+| _ -> begin
+false
+end))
+
+
+let simps : BoolExp.l__BoolExp  ->  BoolExp.l__BoolExp = (fun ( bexp  :  BoolExp.l__BoolExp ) -> (BoolExp.simplify (BoolExp.distributeAnds bexp)))
+
+
+let rec allocN : (ExprTypes.l__GExpr Prims.list * l__BExpState)  ->  Prims.int  ->  (ExprTypes.l__GExpr Prims.list * l__BExpState) = (fun ( _18_494  :  (ExprTypes.l__GExpr Prims.list * l__BExpState) ) ( i  :  Prims.int ) -> (match (_18_494) with
+| (locs, (top, st)) -> begin
+if (i <= 0) then begin
+((FStar.List.rev locs), (top, st))
+end else begin
+(allocN ((ExprTypes.LOC (top))::locs, ((top + 1), (Total.update st top (BoolExp.BVar (top))))) (i - 1))
+end
+end))
+
+
+let allocTy : ExprTypes.l__GType  ->  l__BExpState  ->  (ExprTypes.l__GExpr * l__BExpState) Util.result = (fun ( ty  :  ExprTypes.l__GType ) ( _18_499  :  l__BExpState ) -> (match (_18_499) with
+| (top, st) -> begin
+(match (ty) with
+| ExprTypes.GBool -> begin
+Util.Val ((ExprTypes.LOC (top), ((top + 1), (Total.update st top (BoolExp.BVar (top))))))
+end
+| ExprTypes.GArray (n) -> begin
+(
+
+let _18_505 = (allocN ([], (top, st)) n)
+in (match (_18_505) with
+| (locs, st') -> begin
+Util.Val ((ExprTypes.ARRAY (locs), st'))
+end))
+end
+| _18_507 -> begin
+Util.Err ("Invalid parameter type for circuit generation")
+end)
+end))
+
+
+let rec lookupLst : ExprTypes.l__GExpr Prims.list  ->  l__BExpState  ->  BoolExp.l__BoolExp Prims.list = (fun ( lst  :  ExprTypes.l__GExpr Prims.list ) ( st  :  l__BExpState ) -> (match (lst) with
+| [] -> begin
+[]
+end
+| ExprTypes.LOC (l)::xs -> begin
+((Total.lookup (Prims.snd st) l))::(lookupLst xs st)
+end))
+
+
+let foldPebble : (AncillaHeap.l__AncHeap * Prims.int Prims.list * Prims.int Prims.list * Circuit.l__Gate Prims.list)  ->  BoolExp.l__BoolExp  ->  (AncillaHeap.l__AncHeap * Prims.int Prims.list * Prims.int Prims.list * Circuit.l__Gate Prims.list) = (fun ( _18_522  :  (AncillaHeap.l__AncHeap * Prims.int Prims.list * Prims.int Prims.list * Circuit.l__Gate Prims.list) ) ( bexp  :  BoolExp.l__BoolExp ) -> (match (_18_522) with
+| (ah, outs, anc, circ) -> begin
+(
+
+let _18_528 = (BoolExp.compileBexpPebbled_oop ah (simps bexp))
+in (match (_18_528) with
+| (ah', res, anc', circ') -> begin
+(ah', (res)::outs, (FStar.List.append anc' anc), (FStar.List.append circ circ'))
+end))
+end))
+
+
+let foldClean : (AncillaHeap.l__AncHeap * Prims.int Prims.list * Prims.int Prims.list * Circuit.l__Gate Prims.list)  ->  BoolExp.l__BoolExp  ->  (AncillaHeap.l__AncHeap * Prims.int Prims.list * Prims.int Prims.list * Circuit.l__Gate Prims.list) = (fun ( _18_533  :  (AncillaHeap.l__AncHeap * Prims.int Prims.list * Prims.int Prims.list * Circuit.l__Gate Prims.list) ) ( bexp  :  BoolExp.l__BoolExp ) -> (match (_18_533) with
+| (ah, outs, anc, circ) -> begin
+(
+
+let _18_539 = (BoolExp.compileBexpClean_oop ah (simps bexp))
+in (match (_18_539) with
+| (ah', res, anc', circ') -> begin
+(ah', (res)::outs, (FStar.List.append anc' anc), (FStar.List.append circ circ'))
+end))
+end))
+
+
+let foldBennett : (AncillaHeap.l__AncHeap * Prims.int Prims.list * Prims.int Prims.list * Circuit.l__Gate Prims.list * Circuit.l__Gate Prims.list)  ->  BoolExp.l__BoolExp  ->  (AncillaHeap.l__AncHeap * Prims.int Prims.list * Prims.int Prims.list * Circuit.l__Gate Prims.list * Circuit.l__Gate Prims.list) = (fun ( _18_545  :  (AncillaHeap.l__AncHeap * Prims.int Prims.list * Prims.int Prims.list * Circuit.l__Gate Prims.list * Circuit.l__Gate Prims.list) ) ( bexp  :  BoolExp.l__BoolExp ) -> (match (_18_545) with
+| (ah, outs, anc, circ, ucirc) -> begin
+(
+
+let _18_551 = (BoolExp.compileBexp_oop ah (simps bexp))
+in (match (_18_551) with
+| (ah', res, anc', circ') -> begin
+(ah', (res)::outs, (FStar.List.append anc' anc), (FStar.List.append circ circ'), (FStar.List.append (FStar.List.rev (Circuit.uncompute circ' res)) ucirc))
+end))
+end))
+
+
+let rec compile : l__BExpState config  ->  l__CleanupStrategy  ->  (Prims.int Prims.list * Circuit.l__Gate Prims.list) Util.result = (fun ( _18_554  :  l__BExpState config ) ( strategy  :  l__CleanupStrategy ) -> (match (_18_554) with
+| (gexp, st) -> begin
+if (isVal gexp) then begin
+(match (gexp) with
+| ExprTypes.UNIT -> begin
+Util.Val (([], []))
+end
+| ExprTypes.LAMBDA (x, ty, t) -> begin
+(match ((allocTy ty st)) with
+| Util.Err (s) -> begin
+Util.Err (s)
+end
+| Util.Val (v, st') -> begin
+(compile ((ExprTypes.substGExpr t x v), st') strategy)
+end)
+end
+| ExprTypes.LOC (l) -> begin
+(
+
+let bexp = (Total.lookup (Prims.snd st) l)
+in (
+
+let max = (BoolExp.varMax bexp)
+in (
+
+let _18_579 = (match (strategy) with
+| Pebbled -> begin
+(BoolExp.compileBexpPebbled_oop (AncillaHeap.above (max + 1)) (simps bexp))
+end
+| Boundaries -> begin
+(BoolExp.compileBexpClean_oop (AncillaHeap.above (max + 1)) (simps bexp))
+end
+| Bennett -> begin
+(BoolExp.compileBexpClean_oop (AncillaHeap.above (max + 1)) (simps bexp))
+end)
+in (match (_18_579) with
+| (ah, res, anc, circ) -> begin
+Util.Val (((res)::[], circ))
+end))))
+end
+| ExprTypes.ARRAY (lst) -> begin
+(
+
+let blst = (lookupLst lst st)
+in (
+
+let max = (BoolExp.listMax (FStar.List.mapT BoolExp.varMax blst))
+in (
+
+let _18_607 = (match (strategy) with
+| Pebbled -> begin
+(
+
+let _18_589 = (FStar.List.fold_leftT foldPebble ((AncillaHeap.above (max + 1)), [], [], []) blst)
+in (match (_18_589) with
+| (ah, outs, anc, circ) -> begin
+(ah, (FStar.List.rev outs), (FStar.List.rev anc), circ)
+end))
+end
+| Boundaries -> begin
+(
+
+let _18_595 = (FStar.List.fold_leftT foldClean ((AncillaHeap.above (max + 1)), [], [], []) blst)
+in (match (_18_595) with
+| (ah, outs, anc, circ) -> begin
+(ah, (FStar.List.rev outs), (FStar.List.rev anc), circ)
+end))
+end
+| Bennett -> begin
+(
+
+let _18_602 = (FStar.List.fold_leftT foldBennett ((AncillaHeap.above (max + 1)), [], [], [], []) blst)
+in (match (_18_602) with
+| (ah, outs, anc, circ, ucirc) -> begin
+(ah, (FStar.List.rev outs), (FStar.List.rev anc), (FStar.List.append circ ucirc))
+end))
+end)
+in (match (_18_607) with
+| (ah, outs, anc, circ) -> begin
+Util.Val ((outs, circ))
+end))))
+end)
+end else begin
+(match ((step (gexp, st) bexpInterp)) with
+| Util.Err (s) -> begin
+Util.Err (s)
+end
+| Util.Val (c') -> begin
+(compile c' strategy)
+end)
+end
+end))
+
+
+type circState =
+{top : Prims.int; ah : AncillaHeap.l__AncHeap; gates : Circuit.l__Gate Prims.list; subs : (Prims.int, Prims.int) Total.map}
+
+
+let is_MkcircState : circState  ->  Prims.bool = (Prims.checked_cast(fun ( _  :  circState ) -> (FStar.All.failwith "Not yet implemented:is_MkcircState")))
+
+
+let circInit : circState = {top = 0; ah = AncillaHeap.emptyHeap; gates = []; subs = (Total.const 0)}
+
+
+let circAlloc : circState  ->  BoolExp.l__BoolExp  ->  (Prims.int * circState) = (fun ( cs  :  circState ) ( bexp  :  BoolExp.l__BoolExp ) -> (
+
+let _18_623 = (BoolExp.compileBexp_oop cs.ah (BoolExp.substVar bexp cs.subs))
+in (match (_18_623) with
+| (ah', res, ancs, circ') -> begin
+(
+
+let top' = (cs.top + 1)
+in (
+
+let gates' = (FStar.List.append cs.gates circ')
+in (
+
+let subs' = (Total.update cs.subs cs.top res)
+in (cs.top, {top = top'; ah = ah'; gates = gates'; subs = subs'}))))
+end)))
+
+
+let circAssign : circState  ->  Prims.int  ->  BoolExp.l__BoolExp  ->  circState = (fun ( cs  :  circState ) ( l  :  Prims.int ) ( bexp  :  BoolExp.l__BoolExp ) -> (
+
+let l' = (Total.lookup cs.subs l)
+in (
+
+let bexp' = (BoolExp.substVar bexp cs.subs)
+in (
+
+let _18_639 = (match ((BoolExp.factorAs bexp' l')) with
+| None -> begin
+(BoolExp.compileBexp_oop cs.ah bexp')
+end
+| Some (bexp'') -> begin
+(BoolExp.compileBexp cs.ah l' bexp'')
+end)
+in (match (_18_639) with
+| (ah', res, ancs, circ') -> begin
+{top = cs.top; ah = ah'; gates = (FStar.List.append cs.gates circ'); subs = (Total.update cs.subs l res)}
+end)))))
+
+
+let circEval : circState  ->  Total.state  ->  Prims.int  ->  Prims.bool = (fun ( cs  :  circState ) ( ivals  :  Total.state ) ( i  :  Prims.int ) -> (Circuit.evalCirc cs.gates ivals (Total.lookup cs.subs i)))
+
+
+let circInterp : circState interpretation = {alloc = circAlloc; assign = circAssign; eval = circEval}
+
+
+let rec allocNcirc : (ExprTypes.l__GExpr Prims.list * circState)  ->  Prims.int  ->  (ExprTypes.l__GExpr Prims.list * circState) = (fun ( _18_646  :  (ExprTypes.l__GExpr Prims.list * circState) ) ( i  :  Prims.int ) -> (match (_18_646) with
+| (locs, cs) -> begin
+if (i <= 0) then begin
+((FStar.List.rev locs), cs)
+end else begin
+(
+
+let _18_650 = (AncillaHeap.popMin cs.ah)
+in (match (_18_650) with
+| (ah', res) -> begin
+(
+
+let cs' = {top = (cs.top + 1); ah = ah'; gates = cs.gates; subs = (Total.update cs.subs cs.top res)}
+in (allocNcirc ((ExprTypes.LOC (cs.top))::locs, cs') (i - 1)))
+end))
+end
+end))
+
+
+let allocTycirc : ExprTypes.l__GType  ->  circState  ->  (ExprTypes.l__GExpr * circState) Util.result = (fun ( ty  :  ExprTypes.l__GType ) ( cs  :  circState ) -> (match (ty) with
+| ExprTypes.GBool -> begin
+(
+
+let _18_657 = (AncillaHeap.popMin cs.ah)
+in (match (_18_657) with
+| (ah', res) -> begin
+(
+
+let cs' = {top = (cs.top + 1); ah = ah'; gates = cs.gates; subs = (Total.update cs.subs cs.top res)}
+in Util.Val ((ExprTypes.LOC (cs.top), cs')))
+end))
+end
+| ExprTypes.GArray (n) -> begin
+(
+
+let _18_663 = (allocNcirc ([], cs) n)
+in (match (_18_663) with
+| (locs, st') -> begin
+Util.Val ((ExprTypes.ARRAY (locs), st'))
+end))
+end
+| _18_665 -> begin
+Util.Err ("Invalid parameter type for circuit generation")
+end))
+
+
+let rec lookup_Lst : (Prims.int, Prims.int) Total.map  ->  ExprTypes.l__GExpr Prims.list  ->  Prims.int Prims.list = (fun ( st  :  (Prims.int, Prims.int) Total.map ) ( lst  :  ExprTypes.l__GExpr Prims.list ) -> (match (lst) with
+| [] -> begin
+[]
+end
+| ExprTypes.LOC (l)::xs -> begin
+((Total.lookup st l))::(lookup_Lst st xs)
+end))
+
+
+let rec compileCirc : circState config  ->  (Prims.int Prims.list * Circuit.l__Gate Prims.list) Util.result = (fun ( _18_678  :  circState config ) -> (match (_18_678) with
+| (gexp, cs) -> begin
+if (isVal gexp) then begin
+(match (gexp) with
+| ExprTypes.UNIT -> begin
+Util.Val (([], []))
+end
+| ExprTypes.LAMBDA (x, ty, t) -> begin
+(match ((allocTycirc ty cs)) with
+| Util.Err (s) -> begin
+Util.Err (s)
+end
+| Util.Val (v, cs') -> begin
+(compileCirc ((ExprTypes.substGExpr t x v), cs'))
+end)
+end
+| ExprTypes.LOC (l) -> begin
+(
+
+let res = (Total.lookup cs.subs l)
+in Util.Val (((res)::[], cs.gates)))
+end
+| ExprTypes.ARRAY (lst) -> begin
+(
+
+let res = (lookup_Lst cs.subs lst)
+in Util.Val ((res, cs.gates)))
+end)
+end else begin
+(match ((step (gexp, cs) circInterp)) with
+| Util.Err (s) -> begin
+Util.Err (s)
+end
+| Util.Val (c') -> begin
+(compileCirc c')
+end)
+end
+end))
+
+
+let rec eval_bexp_swap : boolState  ->  l__BExpState  ->  BoolExp.l__BoolExp  ->  Total.state  ->  Prims.unit = (fun ( st  :  boolState ) ( st'  :  l__BExpState ) ( bexp  :  BoolExp.l__BoolExp ) ( init  :  Total.state ) -> ())
+
+
+let state_equiv_alloc : boolState  ->  l__BExpState  ->  Total.state  ->  BoolExp.l__BoolExp  ->  Prims.unit = (fun ( st  :  boolState ) ( st'  :  l__BExpState ) ( init  :  Total.state ) ( bexp  :  BoolExp.l__BoolExp ) -> ())
+
+
+let state_equiv_assign : boolState  ->  l__BExpState  ->  Total.state  ->  Prims.int  ->  BoolExp.l__BoolExp  ->  Prims.unit = (fun ( st  :  boolState ) ( st'  :  l__BExpState ) ( init  :  Total.state ) ( l  :  Prims.int ) ( bexp  :  BoolExp.l__BoolExp ) -> ())
+
+
+let rec state_equiv_step : ExprTypes.l__GExpr  ->  boolState  ->  l__BExpState  ->  Total.state  ->  Prims.unit = (fun ( gexp  :  ExprTypes.l__GExpr ) ( st  :  boolState ) ( st'  :  l__BExpState ) ( init  :  Total.state ) -> ())
+and state_equiv_step_lst : ExprTypes.l__GExpr Prims.list  ->  boolState  ->  l__BExpState  ->  Total.state  ->  Prims.unit = (fun ( lst  :  ExprTypes.l__GExpr Prims.list ) ( st  :  boolState ) ( st'  :  l__BExpState ) ( init  :  Total.state ) -> ())
+
+
+let rec eval_bexp_swap2 : boolState  ->  circState  ->  BoolExp.l__BoolExp  ->  BoolExp.l__BoolExp  ->  Total.state  ->  Prims.unit = (fun ( st  :  boolState ) ( cs  :  circState ) ( bexp  :  BoolExp.l__BoolExp ) ( bexp'  :  BoolExp.l__BoolExp ) ( init  :  Total.state ) -> ())
+
+
+let eval_commutes_subst_circ : boolState  ->  circState  ->  BoolExp.l__BoolExp  ->  BoolExp.l__BoolExp  ->  Total.state  ->  Prims.int  ->  Prims.int  ->  Prims.unit = (fun ( st  :  boolState ) ( cs  :  circState ) ( bexp  :  BoolExp.l__BoolExp ) ( bexp'  :  BoolExp.l__BoolExp ) ( init  :  Total.state ) ( targ  :  Prims.int ) ( targ'  :  Prims.int ) -> ())
+
+
+let eval_commutes_subst_circ_oop : boolState  ->  circState  ->  BoolExp.l__BoolExp  ->  BoolExp.l__BoolExp  ->  Total.state  ->  Prims.unit = (fun ( st  :  boolState ) ( cs  :  circState ) ( bexp  :  BoolExp.l__BoolExp ) ( bexp'  :  BoolExp.l__BoolExp ) ( init  :  Total.state ) -> ())
+
+
+let circ_equiv_alloc : boolState  ->  circState  ->  Total.state  ->  BoolExp.l__BoolExp  ->  Prims.unit = (fun ( st  :  boolState ) ( cs  :  circState ) ( init  :  Total.state ) ( bexp  :  BoolExp.l__BoolExp ) -> ())
+
+
+let circ_equiv_assign : boolState  ->  circState  ->  Total.state  ->  Prims.int  ->  BoolExp.l__BoolExp  ->  Prims.unit = (fun ( st  :  boolState ) ( cs  :  circState ) ( init  :  Total.state ) ( l  :  Prims.int ) ( bexp  :  BoolExp.l__BoolExp ) -> ())
+
+
+let rec circ_equiv_step : ExprTypes.l__GExpr  ->  boolState  ->  circState  ->  Total.state  ->  Prims.unit = (fun ( gexp  :  ExprTypes.l__GExpr ) ( st  :  boolState ) ( st'  :  circState ) ( init  :  Total.state ) -> ())
+and circ_equiv_step_lst : ExprTypes.l__GExpr Prims.list  ->  boolState  ->  circState  ->  Total.state  ->  Prims.unit = (fun ( lst  :  ExprTypes.l__GExpr Prims.list ) ( st  :  boolState ) ( st'  :  circState ) ( init  :  Total.state ) -> ())
+
+
+
+
