src/fs/PairHeap.fs
@@ -1,0 +1,188 @@
+#light "off"
+module PairHeap
+open Prims
+
+type 'a heap =
+| Empty
+| Heap of ('a * 'a heap Prims.list)
+
+
+let is_Empty = (fun ( _  :  obj ) ( _discr_  :  obj ) -> (match (_discr_) with
+| Empty (_) -> begin
+true
+end
+| _ -> begin
+false
+end))
+
+
+let is_Heap = (fun ( _  :  obj ) ( _discr_  :  obj ) -> (match (_discr_) with
+| Heap (_) -> begin
+true
+end
+| _ -> begin
+false
+end))
+
+
+let ___Heap____0 = (fun ( projectee  :  'a heap ) -> (match (projectee) with
+| Heap (_13_4) -> begin
+_13_4
+end))
+
+
+type intHeap =
+Prims.int heap
+
+
+let subheaps : intHeap  ->  intHeap Prims.list = (fun ( hp  :  intHeap ) -> (match (hp) with
+| Heap (r, lst) -> begin
+lst
+end))
+
+
+let merge : intHeap  ->  intHeap  ->  intHeap = (fun ( hp1  :  intHeap ) ( hp2  :  intHeap ) -> (match ((hp1, hp2)) with
+| (Empty, _13_16) -> begin
+hp2
+end
+| (_13_19, Empty) -> begin
+hp1
+end
+| (Heap (r1, h1), Heap (r2, h2)) -> begin
+if (r1 = r2) then begin
+Heap ((r1, (FStar.List.append h2 h1)))
+end else begin
+if (r1 < r2) then begin
+Heap ((r1, (hp2)::h1))
+end else begin
+Heap ((r2, (hp1)::h2))
+end
+end
+end))
+
+
+let insert : intHeap  ->  Prims.int  ->  intHeap = (fun ( hp  :  intHeap ) ( i  :  Prims.int ) -> (merge hp (Heap ((i, [])))))
+
+
+let rec mergePairs : intHeap Prims.list  ->  intHeap = (fun ( hplst  :  intHeap Prims.list ) -> (match (hplst) with
+| [] -> begin
+Empty
+end
+| x::[] -> begin
+x
+end
+| x::y::xs -> begin
+(merge (merge x y) (mergePairs xs))
+end))
+
+
+let deleteMin : intHeap  ->  intHeap = (fun ( hp  :  intHeap ) -> (match (hp) with
+| Heap (_13_47, lst) -> begin
+(mergePairs lst)
+end))
+
+
+let getMin : intHeap  ->  Prims.int = (fun ( hp  :  intHeap ) -> (match (hp) with
+| Heap (r, _13_56) -> begin
+r
+end))
+
+
+let rec mem : Prims.int  ->  intHeap  ->  Prims.bool = (fun ( i  :  Prims.int ) ( hp  :  intHeap ) -> (match (hp) with
+| Empty -> begin
+false
+end
+| Heap (r, lst) -> begin
+((i = r) || (mem_lst i lst))
+end))
+and mem_lst : Prims.int  ->  intHeap Prims.list  ->  Prims.bool = (fun ( i  :  Prims.int ) ( lst  :  intHeap Prims.list ) -> (match (lst) with
+| [] -> begin
+false
+end
+| x::xs -> begin
+((mem i x) || (mem_lst i xs))
+end))
+
+
+let elts : intHeap  ->  Prims.int Util.set = (fun ( hp  :  intHeap ) ( i  :  Prims.int ) -> (mem i hp))
+
+
+let leq_heap : Prims.int  ->  intHeap  ->  Prims.bool = (fun ( i  :  Prims.int ) ( hp  :  intHeap ) -> (match (hp) with
+| Empty -> begin
+true
+end
+| Heap (j, _13_83) -> begin
+(i < j)
+end))
+
+
+let rec is_heap : intHeap  ->  Prims.bool = (fun ( hp  :  intHeap ) -> (match (hp) with
+| Empty -> begin
+true
+end
+| Heap (i, lst) -> begin
+((is_heap_list lst) && (FStar.List.for_allT (leq_heap i) lst))
+end))
+and is_heap_list : intHeap Prims.list  ->  Prims.bool = (fun ( lst  :  intHeap Prims.list ) -> (match (lst) with
+| [] -> begin
+true
+end
+| x::xs -> begin
+((is_heap x) && (is_heap_list xs))
+end))
+
+
+let rec is_heap_app : intHeap Prims.list  ->  intHeap Prims.list  ->  Prims.unit = (fun ( l1  :  intHeap Prims.list ) ( l2  :  intHeap Prims.list ) -> ())
+
+
+let rec leq_heap_trans : Prims.int  ->  Prims.int  ->  intHeap Prims.list  ->  Prims.unit = (fun ( i  :  Prims.int ) ( j  :  Prims.int ) ( l  :  intHeap Prims.list ) -> ())
+
+
+let rec leq_heap_app : Prims.int  ->  intHeap Prims.list  ->  intHeap Prims.list  ->  Prims.unit = (fun ( i  :  Prims.int ) ( l1  :  intHeap Prims.list ) ( l2  :  intHeap Prims.list ) -> ())
+
+
+let swap_root : intHeap  ->  Prims.int  ->  intHeap = (fun ( h  :  intHeap ) ( i  :  Prims.int ) -> (match (h) with
+| Heap (r, lst) -> begin
+Heap ((i, lst))
+end))
+
+
+let merge_heap : intHeap  ->  intHeap  ->  Prims.unit = (fun ( hp1  :  intHeap ) ( hp2  :  intHeap ) -> ())
+
+
+let insert_heap : intHeap  ->  Prims.int  ->  Prims.unit = (fun ( _13_166  :  intHeap ) ( _13_168  :  Prims.int ) -> ())
+
+
+let rec mergePairs_heap : intHeap Prims.list  ->  Prims.unit = (fun ( lst  :  intHeap Prims.list ) -> ())
+
+
+let deleteMin_heap : intHeap  ->  Prims.unit = (fun ( hp  :  intHeap ) -> ())
+
+
+let leq_tree_trans : Prims.int  ->  Prims.int  ->  Prims.unit = (fun ( i  :  Prims.int ) ( j  :  Prims.int ) -> ())
+
+
+let leq_all_trans : Prims.int  ->  Prims.int  ->  intHeap  ->  Prims.unit = (fun ( i  :  Prims.int ) ( j  :  Prims.int ) ( hp  :  intHeap ) -> ())
+
+
+let rec mem_app : intHeap Prims.list  ->  intHeap Prims.list  ->  Prims.unit = (fun ( l1  :  intHeap Prims.list ) ( l2  :  intHeap Prims.list ) -> ())
+
+
+let mem_merge : intHeap  ->  intHeap  ->  Prims.unit = (fun ( h1  :  intHeap ) ( h2  :  intHeap ) -> ())
+
+
+let rec mem_mergePairs : intHeap Prims.list  ->  Prims.unit = (fun ( l  :  intHeap Prims.list ) -> ())
+
+
+let mem_insert : intHeap  ->  Prims.int  ->  Prims.unit = (fun ( h  :  intHeap ) ( i  :  Prims.int ) -> ())
+
+
+let rec leq_is_min : Prims.int  ->  intHeap  ->  Prims.unit = (fun ( i  :  Prims.int ) ( h  :  intHeap ) -> ())
+and leq_is_min_list : Prims.int  ->  intHeap Prims.list  ->  Prims.unit = (fun ( i  :  Prims.int ) ( l  :  intHeap Prims.list ) -> ())
+
+
+let deleteMin_not_in_heap : intHeap  ->  Prims.unit = (fun ( h  :  intHeap ) -> ())
+
+
+
+
