src/fs/Par.fs
@@ -1,0 +1,92 @@
+#light "off"
+module Par
+open Prims
+
+type ('Akey, 'Avalue) map =
+('Akey * 'Avalue) Prims.list
+
+
+let rec dom = (fun ( mp  :  ('k, 'v) map ) -> (match (mp) with
+| [] -> begin
+(fun ( _12_128  :  'k ) -> false)
+end
+| x::xs -> begin
+(fun ( y  :  'k ) -> (((Prims.fst x) = y) || (dom xs y)))
+end))
+
+
+let rec cod = (fun ( mp  :  ('k, 'v) map ) -> (match (mp) with
+| [] -> begin
+(fun ( _12_138  :  'v ) -> false)
+end
+| x::xs -> begin
+(fun ( y  :  'v ) -> (((Prims.snd x) = y) || (cod xs y)))
+end))
+
+
+let defined = (fun ( m  :  ('k, 'v) map ) ( k  :  'k ) -> (Util.mem k (dom m)))
+
+
+let empty = []
+
+
+let rec find = (fun ( lst  :  ('k, 'v) map ) ( v  :  'k ) -> (match (lst) with
+| [] -> begin
+None
+end
+| (x, y)::xs -> begin
+if (x = v) then begin
+Some (y)
+end else begin
+(find xs v)
+end
+end))
+
+
+let rec lookup = (fun ( lst  :  ('k, 'v) map ) ( v  :  'k ) -> (match (lst) with
+| (x, y)::xs -> begin
+if (x = v) then begin
+y
+end else begin
+(lookup xs v)
+end
+end))
+
+
+let rec lookupT = (fun ( lst  :  ('k, 'v) map ) ( v  :  'k ) ( def  :  'v ) -> (match (lst) with
+| [] -> begin
+def
+end
+| (x, y)::xs -> begin
+if (x = v) then begin
+y
+end else begin
+(lookupT xs v def)
+end
+end))
+
+
+let rec update = (fun ( lst  :  ('k, 'v) map ) ( k  :  'k ) ( v  :  'v ) -> (match (lst) with
+| [] -> begin
+((k, v))::[]
+end
+| (x, y)::xs -> begin
+if (x = k) then begin
+((x, v))::xs
+end else begin
+((x, y))::(update xs k v)
+end
+end))
+
+
+let totalize = (fun ( mp  :  ('Aa, 'Ab) map ) ( def  :  'Ab ) ( k  :  'Aa ) -> (match ((find mp k)) with
+| None -> begin
+def
+end
+| Some (b) -> begin
+b
+end))
+
+
+
+
