src/fs/Partial.fs
@@ -1,0 +1,23 @@
+#light "off"
+module Partial
+open Prims
+
+type ('Aa, 'Ad, 'Ab) map =
+'Aa  ->  'Ab
+
+
+let update = (fun ( d  :  'Aa Util.set ) ( b  :  Prims.unit ) ( map  :  ('Aa, Prims.unit, obj) map ) ( x  :  'Aa ) ( y  :  obj ) ( z  :  'Aa ) -> if (z = x) then begin
+y
+end else begin
+(map z)
+end)
+
+
+let lookup = (fun ( d  :  'Aa Util.set ) ( b  :  Prims.unit ) ( map  :  ('Aa, Prims.unit, obj) map ) ( x  :  'Aa ) -> (map x))
+
+
+let dom = (fun ( d  :  'Aa Util.set ) ( b  :  Prims.unit ) ( m  :  ('Aa, Prims.unit, obj) map ) -> d)
+
+
+
+
