src/fs/Total.fs
@@ -1,0 +1,46 @@
+#light "off"
+module Total
+open Prims
+
+type ('Aa, 'Ab) map =
+'Aa  ->  'Ab
+
+
+type ('Aa, 'Ab, 'Am1, 'Am2) l__Equal =
+('Aa, 'Ab, Prims.unit, Prims.unit) FStar.FunctionalExtensionality.l__FEq
+
+
+let lemma_map_equal_intro = (fun ( m1  :  ('Aa, 'Ab) map ) ( m2  :  ('Aa, 'Ab) map ) -> ())
+
+
+let lemma_map_equal_elim = (fun ( m1  :  ('Aa, 'Ab) map ) ( m2  :  ('Aa, 'Ab) map ) -> ())
+
+
+let lemma_map_equal_refl = (fun ( m1  :  ('Aa, 'Ab) map ) ( m2  :  ('Aa, 'Ab) map ) -> ())
+
+
+let lookup = (fun ( map  :  ('Aa, 'Ab) map ) ( x  :  'Aa ) -> (map x))
+
+
+let update = (fun ( map  :  ('Aa, 'Ab) map ) ( x  :  'Aa ) ( y  :  'Ab ) ( z  :  'Aa ) -> if (z = x) then begin
+y
+end else begin
+(map z)
+end)
+
+
+let compose = (fun ( m  :  ('Aa, 'Ab) map ) ( m'  :  ('Ab, 'Ac) map ) ( i  :  'Aa ) -> (m' (m i)))
+
+
+let const = (fun ( v  :  'Ab ) ( _12_45  :  'Aa ) -> v)
+
+
+type state =
+(Prims.int, Prims.bool) map
+
+
+let agree_on_trans = (fun ( mp  :  ('Aa, 'Ab) map ) ( mp'  :  ('Aa, 'Ab) map ) ( mp''  :  ('Aa, 'Ab) map ) ( s  :  'Aa Util.set ) -> ())
+
+
+
+
