src/fs/Util.fs
@@ -1,0 +1,203 @@
+#light "off"
+module Util
+open Prims
+
+type 'An fin =
+Prims.nat
+
+
+type 'Aa set =
+'Aa  ->  Prims.bool
+
+
+let mem = (fun ( i  :  'Aa ) ( s  :  'Aa set ) -> (s i))
+
+
+let empty = (fun ( _11_13  :  'Aa ) -> false)
+
+
+let singleton = (fun ( a  :  'Aa ) ( b  :  'Aa ) -> (b = a))
+
+
+let union = (fun ( a  :  'Aa set ) ( b  :  'Aa set ) ( c  :  'Aa ) -> ((a c) || (b c)))
+
+
+let intersection = (fun ( a  :  'Aa set ) ( b  :  'Aa set ) ( c  :  'Aa ) -> ((a c) && (b c)))
+
+
+let complement = (fun ( s  :  'Aa set ) ( x  :  'Aa ) -> (not ((s x))))
+
+
+let ins = (fun ( a  :  'Aa ) ( b  :  'Aa set ) -> (union (singleton a) b))
+
+
+type ('Aa, 'As1, 'As2) l__Equal =
+('Aa, Prims.bool, Prims.unit, Prims.unit) FStar.FunctionalExtensionality.l__FEq
+
+
+let lemma_equal_intro = (fun ( s1  :  'Aa set ) ( s2  :  'Aa set ) -> ())
+
+
+let lemma_equal_elim = (fun ( s1  :  'Aa set ) ( s2  :  'Aa set ) -> ())
+
+
+let lemma_equal_refl = (fun ( s1  :  'Aa set ) ( s2  :  'Aa set ) -> ())
+
+
+let subset_trans = (fun ( s  :  'Aa set ) ( s'  :  'Aa set ) ( s''  :  'Aa set ) -> ())
+
+
+let subset_ins = (fun ( i  :  'Aa ) ( s  :  'Aa set ) -> ())
+
+
+let ins_subset_pres = (fun ( i  :  'Aa ) ( s  :  'Aa set ) ( s'  :  'Aa set ) -> ())
+
+
+let disjoint_subset = (fun ( s  :  'Aa set ) ( s'  :  'Aa set ) ( s''  :  'Aa set ) -> ())
+
+
+let disjoint_union = (fun ( s  :  'Aa set ) ( s'  :  'Aa set ) ( s''  :  'Aa set ) -> ())
+
+
+type 'a result =
+| Val of 'a
+| Err of Prims.string
+
+
+let is_Val = (fun ( _  :  obj ) ( _discr_  :  obj ) -> (match (_discr_) with
+| Val (_) -> begin
+true
+end
+| _ -> begin
+false
+end))
+
+
+let is_Err = (fun ( _  :  obj ) ( _discr_  :  obj ) -> (match (_discr_) with
+| Err (_) -> begin
+true
+end
+| _ -> begin
+false
+end))
+
+
+let ___Val____0 = (fun ( projectee  :  'a result ) -> (match (projectee) with
+| Val (_11_90) -> begin
+_11_90
+end))
+
+
+let ___Err____0 = (fun ( projectee  :  'a result ) -> (match (projectee) with
+| Err (_11_93) -> begin
+_11_93
+end))
+
+
+let get_Val = (fun ( r  :  'a result ) -> (match (r) with
+| Val (v) -> begin
+v
+end))
+
+
+let bind = (fun ( v  :  'a result ) ( f  :  'a  ->  'b result ) -> (match (v) with
+| Val (x) -> begin
+(f x)
+end
+| Err (s) -> begin
+Err (s)
+end))
+
+
+let bindT = (fun ( v  :  'a result ) ( f  :  'a  ->  'b result ) -> (match (v) with
+| Val (x) -> begin
+(f x)
+end
+| Err (s) -> begin
+Err (s)
+end))
+
+
+let rec foldM = (fun ( f  :  'a  ->  'b  ->  'a result ) ( a  :  'a ) ( lst  :  'b Prims.list ) -> (match (lst) with
+| [] -> begin
+Val (a)
+end
+| x::xs -> begin
+(bind (f a x) (fun ( res  :  'a ) -> (foldM f res xs)))
+end))
+
+
+let mems = (fun ( l  :  'Aa Prims.list ) ( i  :  'Aa ) -> (FStar.List.mem i l))
+
+
+let rec nthT = (fun ( l  :  'a Prims.list ) ( i  :  Prims.int ) -> (match (l) with
+| x::xs -> begin
+if (i = 0) then begin
+x
+end else begin
+(nthT xs (i - 1))
+end
+end))
+
+
+let rec for_someT = (fun ( f  :  'a  ->  Prims.bool ) ( l  :  'a Prims.list ) -> (match (l) with
+| [] -> begin
+false
+end
+| hd::tl -> begin
+if (f hd) then begin
+true
+end else begin
+(for_someT f tl)
+end
+end))
+
+
+let rec take = (fun ( l  :  'a Prims.list ) ( i  :  Prims.int ) -> if (i <= 0) then begin
+[]
+end else begin
+(match (l) with
+| x::xs -> begin
+(x)::(take xs (i - 1))
+end)
+end)
+
+
+let rec remove = (fun ( l  :  'a Prims.list ) ( i  :  Prims.nat ) -> if (i = 0) then begin
+l
+end else begin
+(match (l) with
+| _11_164::xs -> begin
+(remove xs (i - 1))
+end)
+end)
+
+
+let rec rotate_rec = (fun ( acc  :  'a Prims.list ) ( l  :  'a Prims.list ) ( i  :  Prims.nat ) -> if (i = 0) then begin
+(FStar.List.append acc (FStar.List.rev l))
+end else begin
+(match (l) with
+| x::xs -> begin
+(rotate_rec ((x)::acc) xs (i - 1))
+end)
+end)
+
+
+let rotate = (fun ( l  :  'a Prims.list ) ( i  :  Prims.nat ) -> (
+
+let _11_183 = ()
+in (rotate_rec [] (FStar.List.rev l) i)))
+
+
+let slice = (fun ( l  :  'a Prims.list ) ( i  :  Prims.nat ) ( j  :  Prims.nat ) -> (take (remove l i) ((j - i) + 1)))
+
+
+let rec of_int : Prims.nat  ->  Prims.int  ->  Prims.bool Prims.list = (fun ( i  :  Prims.nat ) ( j  :  Prims.int ) -> if (j <= 0) then begin
+[]
+end else begin
+(((i % 2) = 1))::(of_int (i / 2) (j - 1))
+end)
+
+
+
+
