Makefile
@@ -1,21 +1,17 @@
-VERFILES=Util.fst Maps.fst PairHeap.fst AncillaHeap.fst Circuit.fst BoolExp.fst ExprTypes.fst Interpreter.fst Hack.fst
-EX= ext.fst map.fst io.fst listproperties.fst
-EXLIB = $(addprefix $(FSTAR_HOME)/lib/, $(EX))
-include Makefile.include
+FSTAR_HOME = /home/meamy/Programming/FStar
 
-ML=FunctionalExtensionality.ml Util.ml PairHeap.ml AncillaHeap.ml Circuit.ml BoolExp.ml ExprTypes.ml Interpreter.ml main.ml
-MLFILES = $(addprefix ocaml-src/, $(ML))
-SUPPORTFILES=support.ml
+FSTAR = $(FSTAR_HOME)/bin/fstar.exe
 
-#all: .all.ver
-all: $(VERFILES)
-	$(FSTAR) --z3timeout 60 --admit_fsi Set $(STDLIB) $(EXLIB) $^ --verify_module VerifyHack
+FILES = Util.fst Maps.fst PairHeap.fst AncillaHeap.fst Circuit.fst BoolExp.fst ExprTypes.fst Interpreter.fst
+STDLIB = FStar.FunctionalExtensionality.fst FStar.Set.fst FStar.Heap.fst FStar.ST.fst FStar.All.fst FStar.List.fst FStar.String.fsti
+EX = FStar.Map.fst FStar.IO.fsti FStar.ListProperties.fst
 
-cache: .cache
+SRC = $(addprefix src/, $(FILES))
+LIB = $(addprefix $(FSTAR_HOME)/lib/, $(STDLIB) $(EX))
 
-ocamlcode: $(VERFILES)
-	$(FSTAR) --codegen OCaml --z3timeout 60 --n_cores 4 --admit_fsi Set $(STDLIB) $(EXLIB) $^
-	mv *.ml ocaml-src/
+verify: $(SRC)
+	$(FSTAR) --z3timeout 60 --explicit_deps $(LIB) $^
 
-ocaml: $(MLFILES)
-	cd ocaml-src &&	$(OCAMLOPT) -o rever $(SUPPORTFILES) $(ML) &&	mv rever ../
+fs: $(SRC)
+	$(FSTAR) --admit_smt_queries true --codegen FSharp --use_native_int --explicit_deps $(LIB) $^
+	mv *.fs src/
